_array refinement

examples/pseudo_bool/array/npbc_arrayProgScript.sml
@@ -1,11 +1,11 @@
 (*
   Refine npbc_list to npbc_array
 *)
-open preamble basis npbcTheory npbc_listTheory;
+open preamble basis UnsafeProgTheory UnsafeProofTheory npbcTheory npbc_listTheory;
 
 val _ = new_theory "npbc_arrayProg"
 
-val _ = translation_extends"basisProg";
+val _ = translation_extends"UnsafeProg";
 
 val xlet_autop = xlet_auto >- (TRY( xcon) >> xsimpl)
 
@@ -296,12 +296,11 @@ val check_cutting_alt_arr = process_topdecs`
 val r = translate (lslack_def |> SIMP_RULE std_ss [MEMBER_INTRO, o_DEF]);
 val r = translate (check_contradiction_def |> SIMP_RULE std_ss[LET_DEF]);
 
-(* TODO: can use Unsafe.update instead of Array.update *)
 val delete_arr = process_topdecs`
   fun delete_arr i fml =
     if Array.length fml <= i then ()
     else
-      (Array.update fml i None)` |> append_prog
+      (Unsafe.update fml i None)` |> append_prog
 
 Theorem delete_arr_spec:
   NUM i iv ∧
@@ -634,6 +633,16 @@ Proof
   xsimpl
 QED
 
+Theorem ARRAY_W8ARRAY_refl:
+  (ARRAY fml fmllsv * W8ARRAY zerosv zeros ==>> ARRAY fml fmllsv * W8ARRAY zerosv zeros ) ∧
+  (W8ARRAY zerosv zeros * ARRAY fml fmllsv ==>> ARRAY fml fmllsv * W8ARRAY zerosv zeros) ∧
+  (ARRAY fml fmllsv * W8ARRAY zerosv zeros ==>> ARRAY fml fmllsv * W8ARRAY zerosv zeros * GC) ∧
+  (ARRAY fml fmllsv * W8ARRAY zerosv zeros ==>> W8ARRAY zerosv zeros * ARRAY fml fmllsv * GC) ∧
+  (W8ARRAY zerosv zeros * ARRAY fml fmllsv ==>> ARRAY fml fmllsv * W8ARRAY zerosv zeros * GC)
+Proof
+  xsimpl
+QED
+
 Theorem opt_update_arr_spec:
   LIST_REL (OPTION_TYPE bconstraint_TYPE) fmlls fmllsv ∧
   (OPTION_TYPE bconstraint_TYPE) c cv ∧
@@ -700,7 +709,7 @@ val rup_pass1_arr = process_topdecs`
       val k = abs i in
       if n < Word8Array.length assg
       then
-        let val v = Word8Array.sub assg n in
+        let val v = Unsafe.w8sub assg n in
           if eq_zw v then
             rup_pass1_arr assg xs (acc + k) ((k,(i,n))::ys) (max m n)
           else
@@ -763,111 +772,468 @@ Proof
   gvs[]
 QED
 
-(* TODO below *)
+Definition mk_flag_def:
+  mk_flag (i: int) =
+  (if 0 ≤ i then 1w else (2w:word8))
+End
+
+val res = translate mk_flag_def;
+
+val rup_pass2_arr = process_topdecs`
+  fun rup_pass2_arr assg max ls l changes =
+    case ls of [] => (False,changes)
+  | (k,(i,n))::ys =>
+    if max < l + k then
+      (Unsafe.w8update assg n (mk_flag i);
+        rup_pass2_arr assg max ys l (n::changes))
+    else
+      rup_pass2_arr assg max ys l changes` |> append_prog;
+
+Theorem rup_pass2_arr_spec:
+  ∀ls lsv changes changesv assg.
+  NUM max maxv ∧
+  LIST_TYPE (PAIR_TYPE NUM (PAIR_TYPE INT NUM)) ls lsv ∧
+  NUM l lv ∧
+  LIST_TYPE NUM changes changesv ∧
+  rup_pass2_list assg max ls l changes =
+    (res2,changes2,assg2,T) ⇒
+  app (p : 'ffi ffi_proj)
+    ^(fetch_v "rup_pass2_arr" (get_ml_prog_state()))
+    [assgv; maxv; lsv; lv; changesv]
+    (W8ARRAY assgv assg)
+    (POSTv v.
+      W8ARRAY assgv assg2 *
+      SEP_EXISTS v1 v2.
+      &(
+        v = Conv NONE [v1; v2] ∧
+        BOOL res2 v1 ∧
+        LIST_TYPE NUM changes2 v2
+      )
+    )
+Proof
+  Induct>>rw[]>>
+  xcf"rup_pass2_arr"(get_ml_prog_state ())>>
+  gvs[LIST_TYPE_def,rup_pass2_list_def]
+  >- (
+    xmatch>>
+    xlet_autop>>xcon>>xsimpl>>
+    EVAL_TAC)>>
+  PairCases_on`h`>>
+  gvs[PAIR_TYPE_def,rup_pass2_list_def]>>
+  xmatch>>
+  rpt xlet_autop>>
+  reverse xif>>gvs[]
+  >- (
+    xapp>>gvs[]>>
+    goal_assum drule>>
+    gvs[])>>
+  rpt(pairarg_tac>>gvs[])>>
+  rpt xlet_autop>>
+  xapp>>
+  xsimpl>>
+  gvs[mk_flag_def]>>
+  goal_assum drule>>
+  simp[LIST_TYPE_def]
+QED
+
+Definition w8z_def:
+  w8z = (0w: word8)
+End
+
+Definition w8o_def:
+  w8o = (1w: word8)
+End
+
+val w8z_v_thm = translate w8z_def;
+val w8o_v_thm = translate w8o_def;
+
+val resize_to_fit = process_topdecs`
+  fun resize_to_fit n assg =
+    if n < Word8Array.length assg
+      then assg
+    else
+     let val arr = Word8Array.array
+      (3* Word8Array.length assg + n + 1) w8z
+        val u = Word8Array.copy assg 0 (Word8Array.length assg) arr 0 in
+        arr
+      end` |> append_prog;
+
+Theorem resize_to_fit_spec:
+  NUM n nv ⇒
+  app (p : 'ffi ffi_proj)
+    ^(fetch_v "resize_to_fit" (get_ml_prog_state()))
+    [nv; assgv]
+    (W8ARRAY assgv assg)
+    (POSTv v. SEP_EXISTS assg2.
+      W8ARRAY v assg2 *
+      &(
+        resize_to_fit n assg = assg2
+      )
+    )
+Proof
+  xcf"resize_to_fit"(get_ml_prog_state ())>>
+  rpt xlet_autop>>
+  xif>>
+  simp[resize_to_fit_def]
+  >-
+    (xvar>>xsimpl)>>
+  assume_tac w8z_v_thm>>
+  rpt xlet_autop>>
+  xvar>>xsimpl>>
+  simp[w8z_def]
+QED
+
+val update_assg_arr = process_topdecs`
+  fun update_assg_arr assg lsn =
+  case lsn of (ls,n) =>
+  case rup_pass1_arr assg ls 0 [] 0 of (max,ls1,m) =>
+    if max < n then (True, [], assg) else
+    let val assg1 = resize_to_fit m assg in
+      case rup_pass2_arr assg1 max ls1 n [] of
+        (res2,changes2) => (res2,changes2,assg1)
+    end` |> append_prog;
+
+Theorem update_assg_arr_spec:
+  constraint_TYPE lsn lsnv ∧
+  update_assg_list assg lsn = (res,new_changes,assg2,T) ⇒
+  app (p : 'ffi ffi_proj)
+    ^(fetch_v "update_assg_arr" (get_ml_prog_state()))
+    [assgv; lsnv]
+    (W8ARRAY assgv assg)
+    (POSTv v.
+      SEP_EXISTS v1 v2 v3.
+      W8ARRAY v3 assg2 *
+      &(
+        v = Conv NONE [v1; v2; v3] ∧
+        BOOL res v1 ∧
+        LIST_TYPE NUM new_changes v2
+      )
+    )
+Proof
+  xcf"update_assg_arr"(get_ml_prog_state ())>>
+  Cases_on`lsn`>>gvs[PAIR_TYPE_def]>>
+  xmatch>>
+  xlet_autop>>
+  gvs[update_assg_list_def]>>
+  rpt(pairarg_tac>>gvs[])>>
+  xlet_auto
+  >- (
+    xsimpl>>
+    simp[LIST_TYPE_def])>>
+  xmatch>>
+  rpt xlet_autop>>
+  xif>>gvs[]
+  >- (
+    rpt xlet_autop>>
+    xcon>>
+    xsimpl>>
+    EVAL_TAC)>>
+  xlet_auto>>
+  xlet_autop>>
+  gvs[]>>
+  xlet_auto
+  >- (
+    xsimpl>>
+    EVAL_TAC)>>
+  xmatch>>
+  xcon>>xsimpl
+QED
+
+val get_rup_constraint_arr = process_topdecs`
+  fun get_rup_constraint_arr b fml n nc =
+  if n = 0 then Some nc
+  else
+    lookup_core_only_arr b fml n` |> append_prog;
+
+Theorem get_rup_constraint_arr_spec:
+  NUM n nv ∧
+  BOOL b bv ∧
+  LIST_REL (OPTION_TYPE bconstraint_TYPE) fmlls fmllsv ∧
+  constraint_TYPE nc ncv
+  ⇒
+  app (p : 'ffi ffi_proj)
+    ^(fetch_v "get_rup_constraint_arr" (get_ml_prog_state()))
+    [bv; fmlv; nv; ncv]
+    (ARRAY fmlv fmllsv)
+    (POSTv v.
+      ARRAY fmlv fmllsv *
+      &(
+        OPTION_TYPE constraint_TYPE
+        (get_rup_constraint_list b fmlls n nc) v))
+Proof
+  xcf"get_rup_constraint_arr"(get_ml_prog_state ())>>
+  xlet_autop>>
+  xif>>gvs[]
+  >- (
+    xcon>>rw[get_rup_constraint_list_def]>>
+    xsimpl>>
+    simp[OPTION_TYPE_def])>>
+  xapp>>
+  xsimpl>>
+  goal_assum drule>>
+  goal_assum drule>>
+  goal_assum drule>>
+  rw[get_rup_constraint_list_def]
+QED
+
+val check_rup_loop_arr = process_topdecs`
+  fun check_rup_loop_arr b nc fml assg all_changes ls =
+  case ls of
+    [] => (False,assg,all_changes)
+  | (n::ns) =>
+    case get_rup_constraint_arr b fml n nc of
+      None => (False,assg,all_changes)
+    | Some c =>
+    case update_assg_arr assg c of (res,new_changes,assg) =>
+    let val all_changes = new_changes @ all_changes in
+      if res then
+        (List.null ns,assg,all_changes)
+      else
+        check_rup_loop_arr b nc fml assg all_changes ns
+    end` |> append_prog;
+
+Theorem check_rup_loop_arr_spec:
+  ∀ns nsv ac acv assg assgv.
+  BOOL b bv ∧
+  constraint_TYPE nc ncv ∧
+  LIST_REL (OPTION_TYPE bconstraint_TYPE) fmlls fmllsv ∧
+  LIST_TYPE NUM ac acv ∧
+  LIST_TYPE NUM ns nsv ∧
+  check_rup_loop_list b nc fmlls assg ac ns =
+    (res,assg1,ac1,T) ⇒
+  app (p : 'ffi ffi_proj)
+    ^(fetch_v "check_rup_loop_arr" (get_ml_prog_state()))
+    [bv; ncv; fmlv; assgv; acv; nsv]
+    (ARRAY fmlv fmllsv * W8ARRAY assgv assg)
+    (POSTv v.
+      ARRAY fmlv fmllsv *
+      SEP_EXISTS v1 v2 v3.
+      W8ARRAY v2 assg1 *
+      &(
+        v = Conv NONE [v1; v2; v3] ∧
+        BOOL res v1 ∧
+        LIST_TYPE NUM ac1 v3
+      )
+    )
+Proof
+  Induct>>rw[]>>
+  xcf"check_rup_loop_arr"(get_ml_prog_state ())>>
+  gvs[LIST_TYPE_def,check_rup_loop_list_def]>>
+  xmatch
+  >- (
+    xlet_autop>>xcon>>xsimpl>>
+    EVAL_TAC)>>
+  xlet_autop>>
+  gvs[AllCaseEqs(),OPTION_TYPE_def]>>
+  xmatch
+  >- (
+    xlet_autop>>
+    xcon>>xsimpl>>
+    EVAL_TAC)>>
+  rpt(pairarg_tac>>gvs[])>>
+  xlet_auto
+  >- (
+    xsimpl>>
+    gvs[AllCaseEqs()])>>
+  xmatch>>
+  xlet_autop>>
+  xif>>gvs[]
+  >- (
+    xlet_autop>>
+    xcon>>xsimpl>>
+    gvs[NULL_EQ])>>
+  xapp>>xsimpl>>
+  goal_assum drule>>
+  xsimpl
+QED
+
+val delete_each = process_topdecs`
+  fun delete_each ns assg =
+  case ns of [] => ()
+  | (n::ns) =>
+    (Unsafe.w8update assg n w8z;
+    delete_each ns assg)` |> append_prog;
+
+Theorem delete_each_spec:
+  ∀ns nsv assg.
+  LIST_TYPE NUM ns nsv ∧
+  delete_each ns assg = (assg',T) ⇒
+  app (p : 'ffi ffi_proj)
+    ^(fetch_v "delete_each" (get_ml_prog_state()))
+    [nsv; assgv]
+    (W8ARRAY assgv assg)
+    (POSTv v.
+      W8ARRAY assgv assg' *
+      &(UNIT_TYPE () v))
+Proof
+  Induct>>rw[]>>
+  xcf"delete_each"(get_ml_prog_state ())>>
+  gvs[delete_each_def,LIST_TYPE_def]>>
+  xmatch>>xsimpl
+  >-
+    (xcon>>xsimpl)>>
+  pairarg_tac>>gvs[]>>
+  assume_tac w8z_v_thm>>
+  xlet_autop>>
+  xapp>>xsimpl>>
+  simp[w8z_def]
+QED
+
+val check_rup_arr = process_topdecs`
+  fun check_rup_arr b nc fml zeros ls =
+    case check_rup_loop_arr b nc fml zeros [] ls of
+     (res,assg1,all_changes1) =>
+      (delete_each all_changes1 assg1;
+      (res,assg1))` |> append_prog;
+
+Theorem check_rup_arr_spec:
+  BOOL b bv ∧
+  constraint_TYPE nc ncv ∧
+  LIST_REL (OPTION_TYPE bconstraint_TYPE) fmlls fmllsv ∧
+  LIST_TYPE NUM ns nsv ∧
+  check_rup_list b nc fmlls zeros ns = (res,zeros',T) ⇒
+  app (p : 'ffi ffi_proj)
+    ^(fetch_v "check_rup_arr" (get_ml_prog_state()))
+    [bv; ncv; fmlv; zerosv; nsv]
+    (ARRAY fmlv fmllsv * W8ARRAY zerosv zeros)
+    (POSTv v.
+      ARRAY fmlv fmllsv *
+      SEP_EXISTS v1 v2.
+      W8ARRAY v2 zeros' *
+      &(
+        v = Conv NONE [v1; v2] ∧
+        BOOL res v1
+      )
+    )
+Proof
+  xcf"check_rup_arr"(get_ml_prog_state ())>>
+  gvs[check_rup_list_def]>>
+  rpt(pairarg_tac>>gvs[])>>
+  xlet_autop>>
+  xlet_auto
+  >- (
+    xsimpl>>
+    EVAL_TAC)>>
+  xmatch>>
+  xlet_autop>>
+  xcon>>xsimpl
+QED
+
 val check_lstep_arr = process_topdecs`
-  fun check_lstep_arr lno step b fml mindel id =
+  fun check_lstep_arr lno step b fml mindel id zeros =
   case step of
     Check n c =>
     (case Array.lookup fml None n of
       None => raise Fail (format_failure lno ("invalid constraint id: " ^ Int.toString n))
     | Some (c',b) =>
-      if c = c' then (fml, (None, id))
+      if c = c' then (fml, (None, (id, zeros)))
       else raise Fail (format_failure lno (err_check_string c c')))
-  | Noop => (fml, (None, id))
+  | Noop => (fml, (None, (id, zeros)))
   | Delete ls =>
       if every_less mindel fml ls then
-        (list_delete_arr ls fml; (fml, (None, id)))
+        (list_delete_arr ls fml; (fml, (None, (id, zeros))))
       else
         raise Fail (format_failure lno ("Deletion not permitted for core constraints and constraint index < " ^ Int.toString mindel))
   | Cutting constr =>
     let val c = check_cutting_arr lno b fml constr in
-      (fml, (Some(c,b),id))
+      (fml, (Some(c,b), (id, zeros)))
     end
-  | Rup c ns => raise Fail (format_failure lno ("RUP not yet implemented"))
+  | Rup c ls =>
+    (case check_rup_arr b (not_1 c) fml zeros (0::ls) of
+      (res,zeros) =>
+      if res then
+         (fml, (Some(c,b), (id, zeros)))
+      else
+        raise Fail (format_failure lno ("Failed to prove by RUP")))
   | Con c pf n =>
     (case opt_update_arr fml (Some (not_1 c,b)) id of
       (fml_not_c,id') =>
-      (case check_lsteps_arr lno pf b fml_not_c id id' of
-        (fml', id') =>
+      (case check_lsteps_arr lno pf b fml_not_c id id' zeros of
+        (fml', (id', zeros)) =>
           if check_contradiction_fml_arr b fml' n then
             let val u = rollback_arr fml' id id' in
-              (fml', (Some (c,b), id'))
+              (fml', (Some (c,b), (id',zeros)))
             end
           else
             raise Fail (format_failure lno ("Subproof did not derive contradiction from index:" ^ Int.toString n))))
   | _ => raise Fail (format_failure lno ("Proof step not supported"))
-  and check_lsteps_arr lno steps b fml mindel id =
+  and check_lsteps_arr lno steps b fml mindel id zeros =
   case steps of
-    [] => (fml, id)
+    [] => (fml, (id, zeros))
   | s::ss =>
-    (case check_lstep_arr lno s b fml mindel id of
-      (fml', (c , id')) =>
+    (case check_lstep_arr lno s b fml mindel id zeros of
+      (fml', (c , (id', zeros))) =>
         (case opt_update_arr fml' c id' of (fml'',id'') =>
-        check_lsteps_arr lno ss b fml'' mindel id''))
+        check_lsteps_arr lno ss b fml'' mindel id'' zeros))
 ` |> append_prog
 
 val NPBC_CHECK_LSTEP_TYPE_def = fetch "-" "NPBC_CHECK_LSTEP_TYPE_def";
 
 Theorem check_lstep_arr_spec_aux:
-  (∀step b fmlls mindel id stepv lno lnov idv fmlv fmllsv mindelv bv.
+  (∀step b fmlls mindel id zeros stepv lno lnov idv fmlv fmllsv mindelv bv zerosv.
   NPBC_CHECK_LSTEP_TYPE step stepv ∧
   BOOL b bv ∧
   NUM lno lnov ∧
   NUM mindel mindelv ∧
   NUM id idv ∧
-  LIST_REL (OPTION_TYPE bconstraint_TYPE) fmlls fmllsv
+  LIST_REL (OPTION_TYPE bconstraint_TYPE) fmlls fmllsv ∧
+  EVERY (λw. w = 0w) zeros
   ⇒
   app (p : 'ffi ffi_proj)
     ^(fetch_v "check_lstep_arr" (get_ml_prog_state()))
-    [lnov; stepv; bv; fmlv; mindelv; idv]
-    (ARRAY fmlv fmllsv)
+    [lnov; stepv; bv; fmlv; mindelv; idv; zerosv]
+    (ARRAY fmlv fmllsv * W8ARRAY zerosv zeros)
     (POSTve
       (λv.
-        SEP_EXISTS fmlv' fmllsv'.
-        ARRAY fmlv' fmllsv' *
+        SEP_EXISTS fmlv' fmllsv' zerosv' zeros'.
+        ARRAY fmlv' fmllsv' * W8ARRAY zerosv' zeros' *
         &(
-          case check_lstep_list step b fmlls mindel id of
+          case check_lstep_list step b fmlls mindel id zeros of
             NONE => F
           | SOME res =>
             PAIR_TYPE (λl v.
               LIST_REL (OPTION_TYPE bconstraint_TYPE) l fmllsv' ∧
               v = fmlv')
-              (PAIR_TYPE (OPTION_TYPE bconstraint_TYPE) NUM) res v
+              (PAIR_TYPE (OPTION_TYPE bconstraint_TYPE)
+              (PAIR_TYPE NUM (λl v. l = zeros' ∧ v = zerosv') )) res v ∧ EVERY (λw. w = 0w) zeros'
           ))
       (λe.
-        SEP_EXISTS fmlv' fmllsv'.
-        ARRAY fmlv' fmllsv' *
+        SEP_EXISTS fmlv' fmllsv' zerosv' zeros'.
+        ARRAY fmlv' fmllsv' * W8ARRAY zerosv' zeros' *
         & (Fail_exn e ∧
-        check_lstep_list step b fmlls mindel id = NONE)))) ∧
-  (∀steps b fmlls mindel id stepsv lno lnov idv fmlv fmllsv mindelv bv.
+        check_lstep_list step b fmlls mindel id zeros = NONE)))) ∧
+  (∀steps b fmlls mindel id zeros stepsv lno lnov idv fmlv fmllsv mindelv bv zerosv.
   LIST_TYPE NPBC_CHECK_LSTEP_TYPE steps stepsv ∧
   BOOL b bv ∧
   NUM lno lnov ∧
   NUM mindel mindelv ∧
   NUM id idv ∧
-  LIST_REL (OPTION_TYPE bconstraint_TYPE) fmlls fmllsv
+  LIST_REL (OPTION_TYPE bconstraint_TYPE) fmlls fmllsv ∧
+  EVERY (λw. w = 0w) zeros
   ⇒
   app (p : 'ffi ffi_proj)
     ^(fetch_v "check_lsteps_arr" (get_ml_prog_state()))
-    [lnov; stepsv; bv; fmlv; mindelv; idv]
-    (ARRAY fmlv fmllsv)
+    [lnov; stepsv; bv; fmlv; mindelv; idv; zerosv]
+    (ARRAY fmlv fmllsv * W8ARRAY zerosv zeros)
     (POSTve
       (λv.
-        SEP_EXISTS fmlv' fmllsv'.
-        ARRAY fmlv' fmllsv' *
+        SEP_EXISTS fmlv' fmllsv' zerosv' zeros'.
+        ARRAY fmlv' fmllsv' * W8ARRAY zerosv' zeros' *
         &(
-          case check_lsteps_list steps b fmlls mindel id of NONE => F
+          case check_lsteps_list steps b fmlls mindel id zeros of
+            NONE => F
           | SOME res =>
             PAIR_TYPE (λl v.
               LIST_REL (OPTION_TYPE bconstraint_TYPE) l fmllsv' ∧
               v = fmlv')
-              NUM res v
+              (PAIR_TYPE NUM (λl v. l = zeros' ∧ v = zerosv') ) res v ∧
+            EVERY (λw. w = 0w) zeros'
           ))
       (λe.
-        SEP_EXISTS fmlv' fmllsv'.
-        ARRAY fmlv' fmllsv' *
+        SEP_EXISTS fmlv' fmllsv' zerosv' zeros'.
+        ARRAY fmlv' fmllsv' * W8ARRAY zerosv' zeros' *
         & (Fail_exn e ∧
-          check_lsteps_list steps b fmlls mindel id = NONE))))
+          check_lsteps_list steps b fmlls mindel id zeros = NONE))))
 Proof
   ho_match_mp_tac check_lstep_list_ind>>
   rw[]>>fs[]
@@ -878,7 +1244,7 @@ Proof
     >- ( (* Delete *)
       fs[NPBC_CHECK_LSTEP_TYPE_def]>>
       xmatch>>
-      xlet_auto>>
+      xlet_autop>>
       reverse IF_CASES_TAC >>
       gs[]>>xif>>
       asm_exists_tac>>simp[]
@@ -887,7 +1253,7 @@ Proof
         simp[check_lstep_list_def]>>
         xraise>>xsimpl>>
         simp[Fail_exn_def]>>
-        metis_tac[ARRAY_refl])>>
+        metis_tac[ARRAY_W8ARRAY_refl])>>
       rpt xlet_autop>>
       xcon>>xsimpl
       >- (
@@ -897,26 +1263,41 @@ Proof
     >- ((* Cutting *)
       fs[NPBC_CHECK_LSTEP_TYPE_def,check_lstep_list_def]>>
       xmatch>>
-      xlet_auto >- (
+      xlet_autop >- (
         xsimpl>>
-        metis_tac[ARRAY_refl])>>
+        metis_tac[ARRAY_W8ARRAY_refl])>>
       rpt xlet_autop>>
       every_case_tac>>fs[]>>
       xcon>>xsimpl>>
       simp[PAIR_TYPE_def,OPTION_TYPE_def]>>
-      metis_tac[ARRAY_refl])
+      metis_tac[ARRAY_W8ARRAY_refl])
     >- ((* Rup *)
       fs[NPBC_CHECK_LSTEP_TYPE_def,check_lstep_list_def]>>
       xmatch>>
       rpt xlet_autop>>
+      pairarg_tac>>gvs[]>>
+      imp_res_tac check_rup_list_pre>>gvs[]>>
+      xlet_auto
+      >- (
+        xsimpl>>
+        simp[LIST_TYPE_def])>>
+      xmatch>>
+      xif>>gvs[]
+      >- (
+        rpt xlet_autop>>
+        xcon>>xsimpl>>
+        simp[PAIR_TYPE_def]>>
+        asm_exists_tac>>simp[OPTION_TYPE_def,PAIR_TYPE_def]>>
+        xsimpl)>>
+      rpt xlet_autop>>
       xraise>>xsimpl>>
-      metis_tac[ARRAY_refl,Fail_exn_def])
+      metis_tac[ARRAY_W8ARRAY_refl,Fail_exn_def])
     >- ( (* Con *)
       fs[NPBC_CHECK_LSTEP_TYPE_def,check_lstep_list_def]>>
       xmatch>>
       rpt xlet_autop>>
       xlet`POSTv v. SEP_EXISTS fmlv' fmllsv'.
-        ARRAY fmlv' fmllsv' *
+        ARRAY fmlv' fmllsv' * W8ARRAY zerosv zeros *
         &(
           PAIR_TYPE
             (λl v.
@@ -926,13 +1307,21 @@ Proof
             (opt_update fmlls (SOME (not p',b)) id) v)`
       >- (
         xapp>>xsimpl>>
-        simp[OPTION_TYPE_def,PAIR_TYPE_def])>>
+        simp[OPTION_TYPE_def,PAIR_TYPE_def]>>
+        rpt(first_x_assum (irule_at Any))>>
+        qexists_tac`SOME (not p', b)`>>
+        simp[OPTION_TYPE_def,PAIR_TYPE_def]>>rw[]>>
+        xsimpl)>>
       fs[PAIR_TYPE_def]>>
       xmatch>>
-      xlet_autop
+      xlet_auto
       >- (
         xsimpl>>
-        metis_tac[ARRAY_refl])>>
+        metis_tac[ARRAY_W8ARRAY_refl]
+      )
+      >- (
+        xsimpl>>
+        metis_tac[ARRAY_W8ARRAY_refl])>>
       pop_assum mp_tac>> TOP_CASE_TAC>>
       fs[]>>
       PairCases_on`x`>>fs[PAIR_TYPE_def]>>
@@ -953,12 +1342,11 @@ Proof
       xif>>asm_exists_tac>>xsimpl>>
       rpt xlet_autop>>
       xraise>>xsimpl>>
-      metis_tac[Fail_exn_def,ARRAY_refl])
+      metis_tac[Fail_exn_def,ARRAY_W8ARRAY_refl])
     >- ( (* Check *)
       fs[NPBC_CHECK_LSTEP_TYPE_def,check_lstep_list_def]>>
       xmatch>>
       rpt xlet_autop>>
-      xlet_auto>>
       `OPTION_TYPE bconstraint_TYPE (any_el n fmlls NONE) v'` by (
          rw[any_el_ALT]>>
          fs[LIST_REL_EL_EQN,OPTION_TYPE_def])>>
@@ -968,7 +1356,7 @@ Proof
         xmatch>>
         rpt xlet_autop>>
         xraise>> xsimpl>>
-        metis_tac[Fail_exn_def,ARRAY_refl]) >>
+        metis_tac[Fail_exn_def,ARRAY_W8ARRAY_refl]) >>
       Cases_on`x`>>fs[PAIR_TYPE_def]>>xmatch>>
       xlet_autop>>
       xif>>rpt xlet_autop
@@ -978,7 +1366,7 @@ Proof
         asm_exists_tac>>xsimpl)>>
       xraise>>
       xsimpl>>
-      metis_tac[Fail_exn_def,ARRAY_refl])
+      metis_tac[Fail_exn_def,ARRAY_W8ARRAY_refl])
     >- ( (*No Op*)
       fs[NPBC_CHECK_LSTEP_TYPE_def,check_lstep_list_def]>>
       xmatch>>
@@ -1001,24 +1389,35 @@ Proof
     xcfs ["check_lstep_arr","check_lsteps_arr"] (get_ml_prog_state ())>>
     fs[LIST_TYPE_def]>>
     xmatch>>
-    rpt xlet_autop
+    rpt xlet_autop>>
+    xlet_auto
+    >- (
+      xsimpl>>rw[]>>
+      metis_tac[ARRAY_W8ARRAY_refl])
     >- (
       xsimpl>>
       rw[]>>simp[Once check_lstep_list_def]>>
-      metis_tac[ARRAY_refl])>>
+      metis_tac[ARRAY_W8ARRAY_refl])>>
     pop_assum mp_tac>>TOP_CASE_TAC>>strip_tac>>
-    PairCases_on`x`>>fs[PAIR_TYPE_def]>>
+    PairCases_on`x`>>gvs[PAIR_TYPE_def]>>
     xmatch>>
-    xlet_autop>>
+    xlet_auto
+    >- (
+      gvs[]>>
+      rename1`W8ARRAY zzzv zzz`>>
+      qexists_tac`W8ARRAY zzzv zzz`>>
+      xsimpl>>
+      metis_tac[ARRAY_refl])>>
     Cases_on`opt_update x0 x1 x2`>>fs[PAIR_TYPE_def]>>
     xmatch>>
     xapp>>xsimpl>>
-    asm_exists_tac>>xsimpl>>
+    first_x_assum (irule_at Any)>>
+    xsimpl>>
     rw[]>>simp[Once check_lstep_list_def]
     >- (
       every_case_tac>>fs[]>>asm_exists_tac>>
       xsimpl)>>
-    metis_tac[ARRAY_refl])
+    metis_tac[ARRAY_W8ARRAY_refl])
 QED
 
 Theorem check_lstep_arr_spec = CONJUNCT1 check_lstep_arr_spec_aux
@@ -1547,57 +1946,61 @@ Proof
 QED
 
 val check_subproofs_arr = process_topdecs`
-  fun check_subproofs_arr lno pfs b fml mindel id =
+  fun check_subproofs_arr lno pfs b fml mindel id zeros =
   case pfs of
-    [] => (fml,id)
+    [] => (fml,(id,zeros))
   | (cnopt,pf)::pfs =>
     (case cnopt of
       None =>
-      (case check_lsteps_arr lno pf b fml mindel id of
-        (fml', id') =>
-          check_subproofs_arr lno pfs b fml' mindel id')
+      (case check_lsteps_arr lno pf b fml mindel id zeros of
+        (fml', (id', zeros')) =>
+        check_subproofs_arr lno pfs b fml' mindel id' zeros')
     | Some (cs,n) =>
       case list_insert_fml_arr cs b id fml of
         (cid, cfml) =>
-        (case check_lsteps_arr lno pf b cfml id cid of
-          (fml', id') =>
+        (case check_lsteps_arr lno pf b cfml id cid zeros of
+          (fml', (id', zeros')) =>
           if check_contradiction_fml_arr b fml' n then
-            let val u = rollback_arr fml' id id' in
-              check_subproofs_arr lno pfs b fml' mindel id'
-            end
+          let val u = rollback_arr fml' id id' in
+            check_subproofs_arr lno pfs b fml' mindel id' zeros'
+          end
           else
             raise Fail (format_failure lno ("Subproof did not derive contradiction from index:" ^ Int.toString n))))` |> append_prog
 
 Theorem check_subproofs_arr_spec:
-  ∀pfs fmlls mindel id pfsv lno lnov idv fmlv fmllsv mindelv b bv.
+  ∀pfs fmlls mindel id pfsv zeros lno lnov idv fmlv fmllsv mindelv b bv zerosv.
   LIST_TYPE (PAIR_TYPE (OPTION_TYPE (PAIR_TYPE (LIST_TYPE constraint_TYPE) NUM)) (LIST_TYPE NPBC_CHECK_LSTEP_TYPE)) pfs pfsv ∧
   BOOL b bv ∧
   NUM lno lnov ∧
   NUM mindel mindelv ∧
   NUM id idv ∧
-  LIST_REL (OPTION_TYPE bconstraint_TYPE) fmlls fmllsv
+  LIST_REL (OPTION_TYPE bconstraint_TYPE) fmlls fmllsv ∧
+  EVERY (λw. w = 0w) zeros
   ⇒
   app (p : 'ffi ffi_proj)
     ^(fetch_v "check_subproofs_arr" (get_ml_prog_state()))
-    [lnov; pfsv; bv; fmlv; mindelv; idv]
-    (ARRAY fmlv fmllsv)
+    [lnov; pfsv; bv; fmlv; mindelv; idv; zerosv]
+    (ARRAY fmlv fmllsv * W8ARRAY zerosv zeros)
     (POSTve
       (λv.
-        SEP_EXISTS fmlv' fmllsv'.
-        ARRAY fmlv' fmllsv' *
+        SEP_EXISTS fmlv' fmllsv' zerosv' zeros'.
+        ARRAY fmlv' fmllsv' * W8ARRAY zerosv' zeros' *
         &(
-          case check_subproofs_list pfs b fmlls mindel id of
-            NONE => F
-          | SOME res =>
-            PAIR_TYPE (λl v.
-              LIST_REL (OPTION_TYPE bconstraint_TYPE) l fmllsv' ∧
-              v = fmlv') NUM res v
-          ))
+        case check_subproofs_list pfs b fmlls mindel id zeros of
+          NONE => F
+        | SOME res =>
+          PAIR_TYPE (λl v.
+            LIST_REL (OPTION_TYPE bconstraint_TYPE) l fmllsv' ∧
+            v = fmlv')
+            (PAIR_TYPE NUM
+            (λl v. l = zeros' ∧ v = zerosv' ∧ EVERY (λw. w = 0w) zeros') )
+            res v
+        ))
       (λe.
-        SEP_EXISTS fmlv' fmllsv'.
-        ARRAY fmlv' fmllsv' *
+        SEP_EXISTS fmlv' fmllsv' zerosv' zeros'.
+        ARRAY fmlv' fmllsv' * W8ARRAY zerosv' zeros' *
         & (Fail_exn e ∧
-          check_subproofs_list pfs b fmlls mindel id = NONE)))
+          check_subproofs_list pfs b fmlls mindel id zeros = NONE)))
 Proof
   Induct>>
   rw[]>>simp[check_subproofs_list_def]>>
@@ -1605,6 +2008,7 @@ Proof
   fs[LIST_TYPE_def]
   >- (
     xmatch>>
+    xlet_autop>>
     xcon>>xsimpl>>
     simp[PAIR_TYPE_def]>>
     asm_exists_tac>>
@@ -1615,27 +2019,36 @@ Proof
   Cases_on`q`>>fs[OPTION_TYPE_def]
   >- (
     xmatch>>
-    xlet_autop
+    xlet_auto
+    >- (
+      xsimpl>>
+      metis_tac[ARRAY_W8ARRAY_refl])
     >- (
       xsimpl>>
       rw[]>>
-      metis_tac[ARRAY_refl])>>
+      metis_tac[ARRAY_W8ARRAY_refl])>>
     pop_assum mp_tac>>
     TOP_CASE_TAC>>
     PairCases_on`x`>>simp[PAIR_TYPE_def]>>rw[]>>
     xmatch>>
     xapp>>
     xsimpl>>
-    metis_tac[])>>
+    metis_tac[ARRAY_W8ARRAY_refl])>>
   Cases_on`x`>>fs[PAIR_TYPE_def]>>
   xmatch>>
-  xlet_autop>>
+  xlet_auto
+  >- (
+    xsimpl>>
+    metis_tac[ARRAY_refl])>>
   pairarg_tac>>fs[PAIR_TYPE_def]>>
   xmatch>>
-  xlet_autop
+  xlet_auto
+  >- (
+    xsimpl>>
+    metis_tac[ARRAY_W8ARRAY_refl])
   >- (
     xsimpl>>rw[]>>
-    metis_tac[ARRAY_refl])>>
+    metis_tac[ARRAY_W8ARRAY_refl])>>
   pop_assum mp_tac>>
   TOP_CASE_TAC>>fs[]>>
   PairCases_on`x`>>simp[PAIR_TYPE_def]>>
@@ -1645,7 +2058,7 @@ Proof
   >- (
     rpt xlet_autop>>
     xraise>>xsimpl>>
-    metis_tac[Fail_exn_def,ARRAY_refl])>>
+    metis_tac[Fail_exn_def,ARRAY_W8ARRAY_refl])>>
   rpt xlet_autop>>
   xapp>>
   xsimpl>>
@@ -1680,13 +2093,12 @@ val res = translate (hash_pair_def |> REWRITE_RULE hash_simps);
 val res = translate (hash_list_def |> REWRITE_RULE hash_simps);
 val res = translate (hash_constraint_def |> REWRITE_RULE hash_simps);
 
-(* TODO: can use Unsafe.update instead *)
 val mk_hashset_arr = process_topdecs`
   fun mk_hashset_arr ps acc =
   case ps of [] => ()
   | p::ps =>
   let val h = hash_constraint p in
-    Array.update acc h (p::(Array.sub acc h));
+    Unsafe.update acc h (p::(Array.sub acc h));
     mk_hashset_arr ps acc
   end` |> append_prog;
 
@@ -1744,7 +2156,7 @@ QED
 val in_hashset_arr = process_topdecs`
   fun in_hashset_arr p hs =
   let val h = hash_constraint p
-    val r = Array.sub hs h in
+    val r = Unsafe.sub hs h in
     mem_constraint p r
   end` |> append_prog;
 
@@ -2066,19 +2478,20 @@ QED
 val r = translate (red_fast_def |> SIMP_RULE std_ss [vec_eq_nil_thm]);
 
 val check_red_arr_fast = process_topdecs`
-  fun check_red_arr_fast lno b fml inds id c pf cid vimap =
+  fun check_red_arr_fast lno b fml inds id c pf cid vimap zeros =
   let
     val nc = not_1 c
     val fml_not_c = Array.updateResize fml None id (Some (nc,b)) in
-     case check_lsteps_arr lno pf b fml_not_c id (id+1) of
-       (fml', id') =>
+     case check_lsteps_arr lno pf b fml_not_c id (id+1) zeros of
+       (fml', (id', zeros')) =>
       if check_contradiction_fml_arr b fml' cid then
         let val u = rollback_arr fml' id id' in
-          (fml', (inds, (vimap, id')))
+          (fml', (inds, (vimap, (id',zeros'))))
         end
       else raise Fail (format_failure lno ("did not derive contradiction from index:" ^ Int.toString cid))
     end` |> append_prog;
 
+val res = translate opt_insert_def;
 val res = translate set_indices_def;
 
 Definition get_indices_pure_def:
@@ -2088,7 +2501,9 @@ Definition get_indices_pure_def:
     if length v = 0 then INL ()
     else INR inds
   | INL (n,_) =>
-    case sptree$lookup n vimap of
+    case vimap of NONE => INR inds
+    | SOME spt =>
+    case sptree$lookup n spt of
       NONE => INL ()
     | SOME inds => INR inds
 End
@@ -2102,7 +2517,7 @@ val get_indices_arr = process_topdecs`
   | Inr inds => reindex_arr fml inds` |> append_prog;
 
 Overload "vimap_TYPE" = ``
-  SPTREE_SPT_TYPE (LIST_TYPE NUM)``
+  OPTION_TYPE (SPTREE_SPT_TYPE (LIST_TYPE NUM))``
 
 Overload "vomap_TYPE" = ``STRING_TYPE``
 
@@ -2127,6 +2542,8 @@ Proof
   xlet_autop>>
   fs[get_indices_pure_def,get_indices_def]>>
   every_case_tac>>fs[SUM_TYPE_def]>>xmatch
+  >-
+    (xapp>>xsimpl)
   >- (
     rpt xlet_autop>>xcon>>
     xsimpl>>
@@ -2137,7 +2554,12 @@ Proof
     rpt xlet_autop>>xcon>>
     xsimpl>>
     simp[PAIR_TYPE_def,LIST_TYPE_def])
-  >> (xapp>>xsimpl)
+  >- (xapp>>xsimpl)
+  >- (
+    rpt xlet_autop>>xcon>>
+    xsimpl>>
+    simp[PAIR_TYPE_def,LIST_TYPE_def])
+  >- (xapp>>xsimpl)
 QED
 
 val r = translate spt_to_vecTheory.prepend_def;
@@ -2157,7 +2579,7 @@ End
 val res = translate print_lno_mini_def; *)
 
 val check_red_arr = process_topdecs`
-  fun check_red_arr lno ord obj b tcb fml inds id c s pfs idopt vimap vomap =
+  fun check_red_arr lno ord obj b tcb fml inds id c s pfs idopt vimap vomap zeros =
   let val s = mk_subst s in
   case red_fast s idopt pfs of
   None =>
@@ -2171,28 +2593,28 @@ val check_red_arr = process_topdecs`
     val rsubs = do_rso ord s c obj vomap
     val cpfs = extract_clauses_arr lno s b fml rsubs pfs []
     val fml_not_c = Array.updateResize fml None id (Some (nc,b)) in
-     case check_subproofs_arr lno cpfs b fml_not_c id (id+1) of
-       (fml', id') =>
+     case check_subproofs_arr lno cpfs b fml_not_c id (id+1) zeros of
+       (fml', (id', zeros')) =>
      (case idopt of
        None =>
        let val u = rollback_arr fml' id id'
            val goals = subst_indexes_arr s bortcb fml' rinds in
            case red_cond_check bortcb fml' inds' nc pfs rsubs goals
              of None =>
-             (fml', (inds', (vimap',id')))
+             (fml', (inds', (vimap', (id', zeros'))))
            | Some err =>
            raise Fail (format_failure_2 lno ("Redundancy subproofs did not cover all subgoals. Info: " ^ err ^ ".") (print_subproofs_err rsubs goals))
        end
     | Some cid =>
       if check_contradiction_fml_arr b fml' cid then
         let val u = rollback_arr fml' id id' in
-           (fml', (inds', (vimap',id')))
+           (fml', (inds', (vimap', (id', zeros'))))
         end
       else raise Fail (format_failure lno ("did not derive contradiction from index:" ^ Int.toString cid)))
   end
   end)
   | Some (pf,cid) =>
-    check_red_arr_fast lno b fml inds id c pf cid vimap
+    check_red_arr_fast lno b fml inds id c pf cid vimap zeros
   end` |> append_prog;
 
 (* Overloads all the _TYPEs that we will reuse *)
@@ -2215,49 +2637,52 @@ Theorem check_red_arr_fast_spec:
   constraint_TYPE c cv ∧
   LIST_TYPE NPBC_CHECK_LSTEP_TYPE pfs pfsv ∧
   NUM cid cidv ∧
-  vimap_TYPE vimap vimapv
+  vimap_TYPE vimap vimapv ∧
+  EVERY (λw. w = 0w) zeros
   ⇒
   app (p : 'ffi ffi_proj)
     ^(fetch_v "check_red_arr_fast" (get_ml_prog_state()))
     [lnov; bv; fmlv; indsv; idv;
-      cv; pfsv; cidv; vimapv]
-    (ARRAY fmlv fmllsv)
+      cv; pfsv; cidv; vimapv; zerosv]
+    (ARRAY fmlv fmllsv * W8ARRAY zerosv zeros)
     (POSTve
       (λv.
-        SEP_EXISTS fmlv' fmllsv'.
-        ARRAY fmlv' fmllsv' *
+        SEP_EXISTS fmlv' fmllsv' zerosv' zeros'.
+        ARRAY fmlv' fmllsv' * W8ARRAY zerosv' zeros' *
         &(
           case check_red_list_fast b fmlls inds id
-              c pfs cid vimap of NONE => F
+              c pfs cid vimap zeros of NONE => F
           | SOME res =>
             PAIR_TYPE (λl v.
               LIST_REL (OPTION_TYPE bconstraint_TYPE) l fmllsv' ∧
               v = fmlv')
               (PAIR_TYPE (LIST_TYPE NUM)
-                (PAIR_TYPE vimap_TYPE NUM)) res v
+                (PAIR_TYPE vimap_TYPE
+                (PAIR_TYPE NUM (λl v. l = zeros' ∧ v = zerosv' ∧ EVERY (λw. w = 0w) zeros') ))) res v
           ))
       (λe.
-        SEP_EXISTS fmlv' fmllsv'.
-        ARRAY fmlv' fmllsv' *
+        SEP_EXISTS fmlv' fmllsv' zerosv' zeros'.
+        ARRAY fmlv' fmllsv' * W8ARRAY zerosv' zeros' *
         & (Fail_exn e ∧
           check_red_list_fast b fmlls inds id
-              c pfs cid vimap = NONE)))
+              c pfs cid vimap zeros = NONE)))
 Proof
   rw[]>>
   xcf "check_red_arr_fast" (get_ml_prog_state ())>>
   rw[check_red_list_fast_def]>>
   rpt xlet_autop>>
-  xlet_auto>>
-  xlet_autop>>
   `LIST_REL (OPTION_TYPE bconstraint_TYPE)
    (update_resize fmlls NONE (SOME (not c,b)) id)
    (update_resize fmllsv (Conv (SOME (TypeStamp "None" 2)) [])
            (Conv (SOME (TypeStamp "Some" 2)) [Conv NONE [v; bv]]) id)` by (
     match_mp_tac LIST_REL_update_resize>>fs[OPTION_TYPE_def,PAIR_TYPE_def])>>
-  xlet_autop
+  xlet_auto
   >- (
     xsimpl>>
-    metis_tac[ARRAY_refl])>>
+    metis_tac[ARRAY_W8ARRAY_refl])
+  >- (
+    xsimpl>>
+    metis_tac[ARRAY_W8ARRAY_refl])>>
   pop_assum mp_tac>>
   TOP_CASE_TAC>>
   PairCases_on`x`>>simp[PAIR_TYPE_def]>>
@@ -2269,10 +2694,10 @@ Proof
     rpt xlet_autop>>
     xcon>>xsimpl>>
     simp[PAIR_TYPE_def]>>
-    metis_tac[ARRAY_refl])>>
+    metis_tac[ARRAY_W8ARRAY_refl])>>
   rpt xlet_autop>>
   xraise>>xsimpl>>
-  metis_tac[ARRAY_refl,Fail_exn_def]
+  metis_tac[ARRAY_W8ARRAY_refl,Fail_exn_def]
 QED
 
 Overload "subst_raw_TYPE" = ``LIST_TYPE (PAIR_TYPE NUM (SUM_TYPE BOOL (PBC_LIT_TYPE NUM)))``
@@ -2291,33 +2716,36 @@ Theorem check_red_arr_spec:
   pfs_TYPE pfs pfsv ∧
   OPTION_TYPE NUM idopt idoptv ∧
   vimap_TYPE vimap vimapv ∧
-  vomap_TYPE vomap vomapv
+  vomap_TYPE vomap vomapv ∧
+  EVERY (λw. w = 0w) zeros
   ⇒
   app (p : 'ffi ffi_proj)
     ^(fetch_v "check_red_arr" (get_ml_prog_state()))
     [lnov; ordv; objv; bv; tcbv; fmlv; indsv; idv;
-      cv; sv; pfsv; idoptv; vimapv; vomapv]
-    (ARRAY fmlv fmllsv)
+      cv; sv; pfsv; idoptv; vimapv; vomapv; zerosv]
+    (ARRAY fmlv fmllsv * W8ARRAY zerosv zeros)
     (POSTve
       (λv.
-        SEP_EXISTS fmlv' fmllsv'.
-        ARRAY fmlv' fmllsv' *
+        SEP_EXISTS fmlv' fmllsv' zerosv' zeros'.
+        ARRAY fmlv' fmllsv' * W8ARRAY zerosv' zeros' *
         &(
           case check_red_list ord obj b tcb fmlls inds id
-              c s pfs idopt vimap vomap of NONE => F
+              c s pfs idopt vimap vomap zeros of
+            NONE => F
           | SOME res =>
             PAIR_TYPE (λl v.
               LIST_REL (OPTION_TYPE bconstraint_TYPE) l fmllsv' ∧
               v = fmlv')
               (PAIR_TYPE (LIST_TYPE NUM)
-                (PAIR_TYPE vimap_TYPE NUM)) res v
+                (PAIR_TYPE vimap_TYPE
+                (PAIR_TYPE NUM (λl v. l = zeros' ∧ v = zerosv'  ∧ EVERY (λw. w = 0w) zeros') ))) res v
           ))
       (λe.
-        SEP_EXISTS fmlv' fmllsv'.
-        ARRAY fmlv' fmllsv' *
+        SEP_EXISTS fmlv' fmllsv' zerosv' zeros'.
+        ARRAY fmlv' fmllsv' * W8ARRAY zerosv' zeros' *
         & (Fail_exn e ∧
           check_red_list ord obj b tcb fmlls inds id
-              c s pfs idopt vimap vomap = NONE)))
+              c s pfs idopt vimap vomap zeros = NONE)))
 Proof
   rw[]>>
   xcf "check_red_arr" (get_ml_prog_state ())>>
@@ -2335,7 +2763,8 @@ Proof
     metis_tac[])>>
   fs[OPTION_TYPE_def]>>
   xmatch>>
-  xlet`POSTv v. ARRAY fmlv fmllsv * &BOOL (b ∨ tcb) v`
+  xlet`POSTv v. ARRAY fmlv fmllsv * W8ARRAY zerosv zeros *
+    &BOOL (b ∨ tcb) v`
   >- (
     xlog>>xsimpl>>rw[]>>fs[]>>
     xvar>>xsimpl)>>
@@ -2349,29 +2778,28 @@ Proof
   qmatch_goalsub_abbrev_tac`ARRAY aa vv`>>
   xlet`(POSTve
     (λv.
-      ARRAY aa vv *
+      ARRAY aa vv * W8ARRAY zerosv zeros *
       &(case extract_clauses_list ss b fmlls
           (do_rso ord ss c obj vomap) pfs [] of
           NONE => F
         | SOME res => LIST_TYPE (PAIR_TYPE (OPTION_TYPE (PAIR_TYPE (LIST_TYPE constraint_TYPE) NUM)) (LIST_TYPE NPBC_CHECK_LSTEP_TYPE)) res v))
   (λe.
-    ARRAY aa vv *
+    ARRAY aa vv * W8ARRAY zerosv zeros *
     & (Fail_exn e ∧
       extract_clauses_list ss b fmlls (do_rso ord ss c obj vomap) pfs [] = NONE)))`
   >- (
     xapp>>xsimpl>>
-    fs[LIST_TYPE_def]>>
-    metis_tac[])
+    rpt(first_x_assum (irule_at Any))>>
+    qexists_tac`[]`>>
+    fs[LIST_TYPE_def])
   >- (
     xsimpl>>
     fs[do_rso_def]>>
-    metis_tac[ARRAY_refl])>>
+    metis_tac[ARRAY_W8ARRAY_refl])>>
   fs[]>>
   pop_assum mp_tac>>TOP_CASE_TAC>>gvs[]>>
   strip_tac>>
   fs[do_rso_def]>>
-  rpt xlet_autop>>
-  xlet_auto>>
   rpt xlet_autop>>
   rename1`_ (not n) vvv`>>
   `LIST_REL (OPTION_TYPE bconstraint_TYPE)
@@ -2379,14 +2807,18 @@ Proof
     (update_resize fmllsv (Conv (SOME (TypeStamp "None" 2)) [])
             (Conv (SOME (TypeStamp "Some" 2)) [Conv NONE [vvv; bv]]) id)` by (
     match_mp_tac LIST_REL_update_resize>>fs[OPTION_TYPE_def,PAIR_TYPE_def])>>
-  xlet_autop
+  xlet_auto
   >- (
     xsimpl>>rw[]>>
     fs[do_rso_def]>>
-    metis_tac[ARRAY_refl])>>
+    metis_tac[ARRAY_W8ARRAY_refl])
+  >- (
+    xsimpl>>rw[]>>
+    fs[do_rso_def]>>
+    metis_tac[ARRAY_W8ARRAY_refl])>>
   pop_assum mp_tac>>
   TOP_CASE_TAC>>fs[]>>
-  rename1`check_subproofs_list _ _ _ _ _ = SOME yyy`>>
+  rename1`check_subproofs_list _ _ _ _ _ _ = SOME yyy`>>
   PairCases_on`yyy`>>simp[PAIR_TYPE_def]>>
   strip_tac>>
   xmatch>>
@@ -2409,7 +2841,7 @@ Proof
       xraise>>
       xsimpl>>
       rw[]>>fs[]>>
-      metis_tac[ARRAY_refl,NOT_EVERY,Fail_exn_def])
+      metis_tac[ARRAY_W8ARRAY_refl,NOT_EVERY,Fail_exn_def])
     )>>
   rpt xlet_autop>>
   reverse xif
@@ -2418,7 +2850,7 @@ Proof
     xraise>>
     xsimpl>>
     rw[]>>fs[]>>
-    metis_tac[ARRAY_refl,NOT_EVERY,Fail_exn_def]) >>
+    metis_tac[ARRAY_W8ARRAY_refl,NOT_EVERY,Fail_exn_def]) >>
   rpt xlet_autop>>
   xcon>>xsimpl>>
   fs[PAIR_TYPE_def]>>
@@ -2426,31 +2858,34 @@ Proof
 QED
 
 val res = translate opt_cons_def;
+val res = translate update_vimap_aux_def;
 val res = translate update_vimap_def;
 
 val check_sstep_arr = process_topdecs`
   fun check_sstep_arr lno step ord obj tcb fml inds id
-    vimap vomap =
+    vimap vomap zeros =
   case step of
     Lstep lstep =>
-    (case check_lstep_arr lno lstep False fml 0 id of
-      (rfml,(c,id')) =>
+    (case check_lstep_arr lno lstep False fml 0 id zeros of
+      (rfml,(c,(id',zeros))) =>
       (case c of
-        None => (rfml,(inds,(vimap,id')))
+        None => (rfml,(inds,(vimap,(id',zeros))))
       | Some cc =>
         (Array.updateResize rfml None id' (Some cc),
           (sorted_insert id' inds,
           (update_vimap vimap id' (fst (fst cc)),
-          id'+1))) ))
+          (id'+1,
+          zeros)))) ))
   | Red c s pfs idopt =>
     (case check_red_arr lno ord obj False tcb
-        fml inds id c s pfs idopt vimap vomap of
-    (fml',(rinds,(vimap',id'))) =>
+        fml inds id c s pfs idopt vimap vomap zeros of
+    (fml',(rinds,(vimap',(id',zeros)))) =>
        (Array.updateResize fml' None id'
           (Some (c,tcb)),
         (sorted_insert id' rinds,
         (update_vimap vimap' id' (fst c),
-        id'+1))))
+        (id'+1,
+        zeros)))))
   ` |> append_prog
 
 val NPBC_CHECK_SSTEP_TYPE_def = theorem "NPBC_CHECK_SSTEP_TYPE_def";
@@ -2465,32 +2900,34 @@ Theorem check_sstep_arr_spec:
   (LIST_TYPE NUM) inds indsv ∧
   NUM id idv ∧
   vimap_TYPE vimap vimapv ∧
-  vomap_TYPE vomap vomapv
+  vomap_TYPE vomap vomapv ∧
+  EVERY (λw. w = 0w) zeros
   ⇒
   app (p : 'ffi ffi_proj)
     ^(fetch_v "check_sstep_arr" (get_ml_prog_state()))
-    [lnov; stepv; ordv; objv; tcbv; fmlv; indsv; idv; vimapv; vomapv]
-    (ARRAY fmlv fmllsv)
+    [lnov; stepv; ordv; objv; tcbv; fmlv; indsv; idv; vimapv; vomapv; zerosv]
+    (ARRAY fmlv fmllsv * W8ARRAY zerosv zeros)
     (POSTve
       (λv.
-        SEP_EXISTS fmlv' fmllsv'.
-        ARRAY fmlv' fmllsv' *
+        SEP_EXISTS fmlv' fmllsv' zerosv' zeros'.
+        ARRAY fmlv' fmllsv' * W8ARRAY zerosv' zeros' *
         &(
           case check_sstep_list step ord obj tcb
-            fmlls inds id vimap vomap of NONE => F
+            fmlls inds id vimap vomap zeros of NONE => F
           | SOME res =>
             PAIR_TYPE (λl v.
               LIST_REL (OPTION_TYPE bconstraint_TYPE) l fmllsv' ∧
               v = fmlv')
               (PAIR_TYPE (LIST_TYPE NUM)
-                (PAIR_TYPE (vimap_TYPE) NUM)) res v)
+                (PAIR_TYPE (vimap_TYPE)
+                (PAIR_TYPE NUM (λl v. l = zeros' ∧ v = zerosv'  ∧ EVERY (λw. w = 0w) zeros') ))) res v)
           )
       (λe.
-        SEP_EXISTS fmlv' fmllsv'.
-        ARRAY fmlv' fmllsv' *
+        SEP_EXISTS fmlv' fmllsv' zerosv' zeros'.
+        ARRAY fmlv' fmllsv' * W8ARRAY zerosv' zeros' *
         & (Fail_exn e ∧
           check_sstep_list step ord obj tcb
-            fmlls inds id vimap vomap = NONE)))
+            fmlls inds id vimap vomap zeros = NONE)))
 Proof
   rw[]>>
   xcf "check_sstep_arr" (get_ml_prog_state ())>>
@@ -2501,29 +2938,30 @@ Proof
     xlet_autop>>
     xlet`POSTve
       (λv.
-        SEP_EXISTS fmlv' fmllsv'.
-        ARRAY fmlv' fmllsv' *
+        SEP_EXISTS fmlv' fmllsv' zerosv' zeros'.
+        ARRAY fmlv' fmllsv' * W8ARRAY zerosv' zeros' *
         &(
-          case check_lstep_list l F fmlls 0 id of
+          case check_lstep_list l F fmlls 0 id zeros of
             NONE => F
           | SOME res =>
             PAIR_TYPE (λl v.
               LIST_REL (OPTION_TYPE bconstraint_TYPE) l fmllsv' ∧
               v = fmlv')
-              (PAIR_TYPE (OPTION_TYPE bconstraint_TYPE) NUM) res v
+              (PAIR_TYPE (OPTION_TYPE bconstraint_TYPE)
+              (PAIR_TYPE NUM (λl v. l = zeros' ∧ v = zerosv') )) res v ∧ EVERY (λw. w = 0w) zeros'
           ))
       (λe.
-        SEP_EXISTS fmlv' fmllsv'.
-        ARRAY fmlv' fmllsv' *
+        SEP_EXISTS fmlv' fmllsv' zerosv' zeros'.
+        ARRAY fmlv' fmllsv' * W8ARRAY zerosv' zeros' *
         & (Fail_exn e ∧
-        check_lstep_list l F fmlls 0 id = NONE))`
+        check_lstep_list l F fmlls 0 id zeros = NONE))`
     >- (
       xapp>>xsimpl>>
       CONJ_TAC >- EVAL_TAC>>
       metis_tac[])
     >- (
       xsimpl>>
-      metis_tac[ARRAY_refl])>>
+      metis_tac[ARRAY_W8ARRAY_refl])>>
     pop_assum mp_tac>>
     TOP_CASE_TAC>>rw[]>>
     PairCases_on`x`>>fs[PAIR_TYPE_def]>>
@@ -2535,9 +2973,8 @@ Proof
       rpt xlet_autop>>
       xcon>>xsimpl>>
       simp[PAIR_TYPE_def,PULL_EXISTS]>>
-      metis_tac[ARRAY_refl])>>
+      metis_tac[ARRAY_W8ARRAY_refl])>>
     rpt xlet_autop>>
-    xlet_auto>>
     xcon>>xsimpl>>
     simp[PAIR_TYPE_def]>>
     qmatch_goalsub_abbrev_tac`ARRAY _ A`>>
@@ -2549,37 +2986,37 @@ Proof
     xmatch>>
     xlet_autop>>
     rename1`check_red_list ord obj F tcb fmlls inds id
-              c s pfs idopt vimap vomap`>>
+              c s pfs idopt vimap vomap zeros`>>
     xlet`POSTve
       (λv.
-        SEP_EXISTS fmlv' fmllsv'.
-        ARRAY fmlv' fmllsv' *
+        SEP_EXISTS fmlv' fmllsv' zerosv' zeros'.
+        ARRAY fmlv' fmllsv' * W8ARRAY zerosv' zeros' *
         &(
           case check_red_list ord obj F tcb fmlls inds id
-              c s pfs idopt vimap vomap of NONE => F
+              c s pfs idopt vimap vomap zeros of NONE => F
           | SOME res =>
             PAIR_TYPE (λl v.
               LIST_REL (OPTION_TYPE bconstraint_TYPE) l fmllsv' ∧
               v = fmlv') (PAIR_TYPE (LIST_TYPE NUM)
-                (PAIR_TYPE vimap_TYPE NUM)) res v
+                (PAIR_TYPE vimap_TYPE
+                (PAIR_TYPE NUM (λl v. l = zeros' ∧ v = zerosv'  ∧ EVERY (λw. w = 0w) zeros') ))) res v
           ))
       (λe.
-        SEP_EXISTS fmlv' fmllsv'.
-        ARRAY fmlv' fmllsv' *
+        SEP_EXISTS fmlv' fmllsv' zerosv' zeros'.
+        ARRAY fmlv' fmllsv' * W8ARRAY zerosv' zeros' *
         & (Fail_exn e ∧
           check_red_list ord obj F tcb fmlls inds id
-              c s pfs idopt vimap vomap = NONE))`
+              c s pfs idopt vimap vomap zeros = NONE))`
     >- (
       xapp >> xsimpl>>
       CONJ_TAC >- EVAL_TAC>>
       metis_tac[])
     >- (
       xsimpl>>
-      metis_tac[ARRAY_refl])>>
+      metis_tac[ARRAY_W8ARRAY_refl])>>
     every_case_tac>>fs[PAIR_TYPE_def]>>
     xmatch>>
     rpt xlet_autop>>
-    xlet_auto>>
     xcon>>xsimpl>>
     match_mp_tac LIST_REL_update_resize>>
     simp[OPTION_TYPE_def,PAIR_TYPE_def]>>
@@ -2614,8 +3051,11 @@ val nn_int_side = Q.prove(
   EVAL_TAC>>
   intLib.ARITH_TAC
   ) |> update_precondition
+val res = translate npbc_checkTheory.rup_pass1_def;
+val res = translate npbc_checkTheory.rup_pass2_def;
 val res = translate npbc_checkTheory.update_assg_def;
 val res = translate npbc_checkTheory.model_bounding_def;
+val res = translate npbc_checkTheory.get_rup_constraint_def;
 val res = translate npbc_checkTheory.check_rup_def;
 val res = translate npbc_checkTheory.check_lstep_def;
 val res = translate npbc_checkTheory.list_insert_fml_def;
@@ -2710,7 +3150,7 @@ Proof
 QED
 
 Definition check_dom_list_def:
-  check_dom_list spo obj fml inds id c s pfs idopt =
+  check_dom_list spo obj fml inds id c s pfs idopt zeros =
   let rinds = reindex fml inds in
   let corels = core_fmlls fml rinds in
   let nc = not c in
@@ -2720,13 +3160,13 @@ Definition check_dom_list_def:
   case extract_clauses_list s F fml dsubs pfs [] of
     NONE => NONE
   | SOME cpfs =>
-    (case check_subproofs_list cpfs F fml_not_c id (id+1) of
+    (case check_subproofs_list cpfs F fml_not_c id (id+1) zeros of
       NONE => NONE
-    | SOME (fml',id') =>
+    | SOME (fml',(id',zeros')) =>
       let rfml = rollback fml' id id' in
       if do_dom_check idopt fml' rfml w
         corels rinds nc pfs dsubs then
-        SOME (rfml,rinds,id')
+        SOME (rfml,rinds,id',zeros')
       else NONE)
 End
 
@@ -2747,7 +3187,7 @@ val res = translate map_snd_def;
 (* TODO: we can defer corels until the split *)
 val check_dom_arr = process_topdecs`
   fun check_dom_arr lno spo obj fml inds
-    id c s pfs idopt =
+    id c s pfs idopt zeros =
     let
     val rinds = reindex_arr fml inds
     val corels = core_fmlls_arr fml rinds
@@ -2756,21 +3196,21 @@ val check_dom_arr = process_topdecs`
     val nc = not_1 c
     val fml_not_c = Array.updateResize fml None id (Some (nc,False)) in
      case check_subproofs_arr lno cpfs False
-      fml_not_c id (id+1) of
-       (fml',id') =>
+      fml_not_c id (id+1) zeros of
+       (fml',(id',zeros')) =>
        (case idopt of
          None =>
          let val u = rollback_arr fml' id id'
              val goals = core_subgoals s corels in
              case red_cond_check False fml' rinds nc pfs dsubs goals of
-               None => (fml',(rinds,id'))
+               None => (fml',(rinds,(id',zeros')))
              | Some err =>
               raise Fail (format_failure_2 lno ("Dominance subproofs did not cover all subgoals. Info: " ^ err ^ ".") (print_subproofs_err dsubs goals))
          end
        | Some cid =>
          if check_contradiction_fml_arr False fml' cid then
            let val u = rollback_arr fml' id id' in
-             (fml', (rinds,id'))
+             (fml', (rinds, (id', zeros')))
            end
          else raise Fail (format_failure lno ("did not derive contradiction from index:" ^ Int.toString cid)))
     end` |> append_prog;
@@ -2785,31 +3225,33 @@ Theorem check_dom_arr_spec:
   constraint_TYPE c cv ∧
   subst_TYPE s sv ∧
   pfs_TYPE pfs pfsv ∧
-  OPTION_TYPE NUM idopt idoptv
+  OPTION_TYPE NUM idopt idoptv ∧
+  EVERY (λw. w = 0w) zeros
   ⇒
   app (p : 'ffi ffi_proj)
     ^(fetch_v "check_dom_arr" (get_ml_prog_state()))
     [lnov; spov; objv; fmlv; indsv; idv;
-      cv; sv; pfsv; idoptv]
-    (ARRAY fmlv fmllsv)
+      cv; sv; pfsv; idoptv;zerosv]
+    (ARRAY fmlv fmllsv * W8ARRAY zerosv zeros)
     (POSTve
       (λv.
-        SEP_EXISTS fmlv' fmllsv'.
-        ARRAY fmlv' fmllsv' *
+        SEP_EXISTS fmlv' fmllsv' zerosv' zeros'.
+        ARRAY fmlv' fmllsv' * W8ARRAY zerosv' zeros' *
         &(
           case check_dom_list spo obj fmlls inds id
-              c s pfs idopt of NONE => F
+              c s pfs idopt zeros of NONE => F
           | SOME res =>
             PAIR_TYPE (λl v.
               LIST_REL (OPTION_TYPE bconstraint_TYPE) l fmllsv' ∧
-              v = fmlv') (PAIR_TYPE (LIST_TYPE NUM) NUM) res v
+              v = fmlv') (PAIR_TYPE (LIST_TYPE NUM)
+              (PAIR_TYPE NUM (λl v. l = zeros' ∧ v = zerosv'  ∧ EVERY (λw. w = 0w) zeros') )) res v
           ))
       (λe.
-        SEP_EXISTS fmlv' fmllsv'.
-        ARRAY fmlv' fmllsv' *
+        SEP_EXISTS fmlv' fmllsv' zerosv' zeros'.
+        ARRAY fmlv' fmllsv' * W8ARRAY zerosv' zeros' *
         & (Fail_exn e ∧
           check_dom_list spo obj fmlls inds id
-              c s pfs idopt = NONE)))
+              c s pfs idopt zeros = NONE)))
 Proof
   rw[]>>
   xcf "check_dom_arr" (get_ml_prog_state ())>>
@@ -2817,29 +3259,30 @@ Proof
   rpt xlet_autop>>
   xlet`(POSTve
     (λv.
-      ARRAY fmlv fmllsv *
+      ARRAY fmlv fmllsv * W8ARRAY zerosv zeros *
       &(case extract_clauses_list s F fmlls
         (do_dso spo s c obj) pfs [] of
           NONE => F
         | SOME res => LIST_TYPE (PAIR_TYPE (OPTION_TYPE (PAIR_TYPE (LIST_TYPE constraint_TYPE) NUM)) (LIST_TYPE NPBC_CHECK_LSTEP_TYPE)) res v))
     (λe.
-      ARRAY fmlv fmllsv *
+      ARRAY fmlv fmllsv * W8ARRAY zerosv zeros *
       & (Fail_exn e ∧ extract_clauses_list s F fmlls
         (do_dso spo s c obj) pfs [] = NONE)))`
   >- (
     xapp>>xsimpl>>
     simp[LIST_TYPE_def]>>
+    rpt(first_x_assum (irule_at Any))>>
+    qexists_tac`F`>>qexists_tac`[]`>>
+    CONJ_TAC >- EVAL_TAC>>
     CONJ_TAC >- EVAL_TAC>>
     metis_tac[])
   >- (
     xsimpl>>
     simp[do_dso_def,check_dom_list_def]>>
-    metis_tac[ARRAY_refl])>>
+    metis_tac[ARRAY_W8ARRAY_refl])>>
   pop_assum mp_tac>>TOP_CASE_TAC>>simp[]>>
   fs[do_dso_def]>>
   strip_tac>>
-  rpt xlet_autop>>
-  xlet_auto>>
   rpt xlet_autop>>
   rename1`_ (not n) vvv`>>
   qmatch_asmsub_abbrev_tac`Conv (SOME (TypeStamp "Some" 2))
@@ -2855,25 +3298,25 @@ Proof
   fs[Abbr`bbb`]>>
   xlet`(POSTve
       (λv.
-        SEP_EXISTS fmlv' fmllsv'.
-        ARRAY fmlv' fmllsv' *
+        SEP_EXISTS fmlv' fmllsv' zerosv' zeros'.
+        ARRAY fmlv' fmllsv' * W8ARRAY zerosv' zeros' *
         &(
           case check_subproofs_list x F
             (update_resize fmlls NONE (SOME (not n,F)) id)
-            id (id+1) of
+            id (id+1) zeros of
             NONE => F
           | SOME res =>
             PAIR_TYPE (λl v.
               LIST_REL (OPTION_TYPE bconstraint_TYPE) l fmllsv' ∧
-              v = fmlv') NUM res v
-          ))
+              v = fmlv')
+            (PAIR_TYPE NUM (λl v. l = zeros' ∧ v = zerosv'  ∧ EVERY (λw. w = 0w) zeros') ) res v))
       (λe.
-        SEP_EXISTS fmlv' fmllsv'.
-        ARRAY fmlv' fmllsv' *
+        SEP_EXISTS fmlv' fmllsv' zerosv' zeros'.
+        ARRAY fmlv' fmllsv' * W8ARRAY zerosv' zeros' *
         & (Fail_exn e ∧
           check_subproofs_list x F
             (update_resize fmlls NONE (SOME (not n,F)) id)
-            id (id+1) = NONE)))`
+            id (id+1) zeros = NONE)))`
   >- (
     xapp>>
     xsimpl>>
@@ -2882,7 +3325,7 @@ Proof
   >- (
     xsimpl>>
     simp[check_dom_list_def]>>
-    metis_tac[ARRAY_refl])>>
+    metis_tac[ARRAY_W8ARRAY_refl])>>
   pop_assum mp_tac>>
   TOP_CASE_TAC>>fs[]>>
   PairCases_on`x'`>>fs[PAIR_TYPE_def]>>
@@ -2894,12 +3337,12 @@ Proof
   >- (
     xlet_autop>>
     xlet_autop>>
-    xlet`POSTv v. ARRAY fmlv' fmllsv'' * & BOOL F v`
+    xlet`POSTv v. ARRAY fmlv' fmllsv'' * W8ARRAY zerosv' zeros' * & BOOL F v`
     >-
       (xcon>>xsimpl)>>
     qmatch_asmsub_abbrev_tac`LIST_REL _ fmlls'' fmllsv''`>>
     xlet`POSTv resv.
-         ARRAY fmlv' fmllsv'' *
+         ARRAY fmlv' fmllsv'' * W8ARRAY zerosv' zeros' *
          & ∃err.
            OPTION_TYPE STRING_TYPE
            (if
@@ -2910,11 +3353,12 @@ Proof
                 NONE
               else SOME err) resv`
     >-
-      (xapp>>xsimpl)>>
+      (xapp>>xsimpl>>
+      metis_tac[])>>
     pop_assum mp_tac>>IF_CASES_TAC>>
     strip_tac>>fs[OPTION_TYPE_def]>>xmatch
     >- (
-      xlet_autop>>
+      rpt xlet_autop>>
       xcon>>xsimpl>>
       pairarg_tac>>fs[red_cond_check_def,core_subgoals_def]>>
       fs[PAIR_TYPE_def,OPTION_TYPE_def]>>
@@ -2924,23 +3368,24 @@ Proof
       fs[red_cond_check_def]>>pairarg_tac>>fs[core_subgoals_def]>>
       xraise>>xsimpl>>
       fs[red_cond_check_def]>>rw[]>>
-      metis_tac[ARRAY_refl,Fail_exn_def,NOT_EVERY])
+      metis_tac[ARRAY_W8ARRAY_refl,Fail_exn_def,NOT_EVERY])
     )>>
   rename1`check_contradiction_fml_list F A B`>>
   xlet_autop>>
   xlet`POSTv v.
-    ARRAY fmlv' fmllsv' * &
-    BOOL (check_contradiction_fml_list F A B) v`
+    ARRAY fmlv' fmllsv' * W8ARRAY zerosv' zeros' *
+    &BOOL (check_contradiction_fml_list F A B) v`
   >- (
     xapp>>xsimpl>>
-    EVAL_TAC)>>
+    rpt(first_x_assum (irule_at Any))>>
+    qexists_tac`F`>>xsimpl)>>
   reverse xif
   >- (
     rpt xlet_autop>>
     xraise>>
     xsimpl>>
     rw[]>>fs[]>>
-    metis_tac[ARRAY_refl,NOT_EVERY,Fail_exn_def])>>
+    metis_tac[ARRAY_W8ARRAY_refl,NOT_EVERY,Fail_exn_def])>>
   rpt xlet_autop>>
   xcon>>xsimpl>>
   simp[PAIR_TYPE_def]>>
@@ -3085,7 +3530,7 @@ val res = translate npbc_checkTheory.mk_diff_obj_def;
 val res = translate npbc_checkTheory.mk_tar_obj_def;
 
 val check_change_obj_arr = process_topdecs `
-  fun check_change_obj_arr lno b fml id obj fc' pfs =
+  fun check_change_obj_arr lno b fml id obj fc' pfs zeros =
   case obj of None =>
     raise Fail (format_failure lno ("no objective to change"))
   | Some fc =>
@@ -3094,11 +3539,11 @@ val check_change_obj_arr = process_topdecs `
     val bb = True
     val e = []
     val cpfs = extract_clauses_arr lno emp_vec bb fml csubs pfs e in
-    case check_subproofs_arr lno cpfs bb fml id id of
-       (fml', id') =>
+    case check_subproofs_arr lno cpfs bb fml id id zeros of
+       (fml', (id', zeros')) =>
       let val u = rollback_arr fml' id id' in
         if do_change_obj_check pfs csubs then
-          (fml',(mk_diff_obj b fc fc',id'))
+          (fml',(mk_diff_obj b fc fc', (id', zeros')))
        else raise Fail (format_failure lno ("Objective change subproofs did not cover all subgoals. Expected: #[1-2]"))
        end
     end` |> append_prog
@@ -3110,31 +3555,32 @@ Theorem check_change_obj_arr_spec:
   NUM id idv ∧
   obj_TYPE obj objv ∧
   (PAIR_TYPE (LIST_TYPE (PAIR_TYPE INT NUM)) INT) fc fcv ∧
-  pfs_TYPE pfs pfsv
+  pfs_TYPE pfs pfsv ∧
+  EVERY (λw. w = 0w) zeros
   ⇒
   app (p : 'ffi ffi_proj)
     ^(fetch_v "check_change_obj_arr" (get_ml_prog_state()))
-    [lnov; bv; fmlv; idv; objv; fcv; pfsv]
-    (ARRAY fmlv fmllsv)
+    [lnov; bv; fmlv; idv; objv; fcv; pfsv; zerosv]
+    (ARRAY fmlv fmllsv * W8ARRAY zerosv zeros)
     (POSTve
       (λv.
-        SEP_EXISTS fmlv' fmllsv'.
-        ARRAY fmlv' fmllsv' *
+        SEP_EXISTS fmlv' fmllsv' zerosv' zeros'.
+        ARRAY fmlv' fmllsv' * W8ARRAY zerosv' zeros' *
         &(
-          case check_change_obj_list b fmlls id obj fc pfs of
+          case check_change_obj_list b fmlls id obj fc pfs zeros of
             NONE => F
           | SOME res =>
             PAIR_TYPE (λl v.
               LIST_REL (OPTION_TYPE bconstraint_TYPE) l fmllsv' ∧
               v = fmlv')
-            (PAIR_TYPE (PAIR_TYPE (LIST_TYPE (PAIR_TYPE INT NUM)) INT) NUM)
-              res v
+            (PAIR_TYPE (PAIR_TYPE (LIST_TYPE (PAIR_TYPE INT NUM)) INT)
+            (PAIR_TYPE NUM (λl v. l = zeros' ∧ v = zerosv'  ∧ EVERY (λw. w = 0w) zeros') )) res v
           ))
       (λe.
-        SEP_EXISTS fmlv' fmllsv'.
-        ARRAY fmlv' fmllsv' *
+        SEP_EXISTS fmlv' fmllsv' zerosv' zeros'.
+        ARRAY fmlv' fmllsv' * W8ARRAY zerosv' zeros' *
         & (Fail_exn e ∧
-          check_change_obj_list b fmlls id obj fc pfs = NONE)))
+          check_change_obj_list b fmlls id obj fc pfs zeros = NONE)))
 Proof
   rw[]>>
   xcf "check_change_obj_arr" (get_ml_prog_state ())>>
@@ -3144,59 +3590,65 @@ Proof
   >- (
     rpt xlet_autop>>
     xraise>>xsimpl>>
-    metis_tac[ARRAY_refl,Fail_exn_def])>>
+    metis_tac[ARRAY_W8ARRAY_refl,Fail_exn_def])>>
   rpt xlet_autop>>
   qmatch_goalsub_abbrev_tac`ARRAY aa vv`>>
   xlet`(POSTve
     (λv.
-      ARRAY aa vv *
+      ARRAY aa vv * W8ARRAY zerosv zeros *
       &(case extract_clauses_list emp_vec T fmlls
           (change_obj_subgoals (mk_tar_obj b x) fc) pfs [] of
           NONE => F
         | SOME res => LIST_TYPE (PAIR_TYPE (OPTION_TYPE (PAIR_TYPE (LIST_TYPE constraint_TYPE) NUM)) (LIST_TYPE NPBC_CHECK_LSTEP_TYPE)) res v))
   (λe.
-    ARRAY aa vv *
+    ARRAY aa vv * W8ARRAY zerosv zeros *
     & (Fail_exn e ∧
       extract_clauses_list emp_vec T fmlls
       (change_obj_subgoals (mk_tar_obj b x) fc) pfs [] = NONE)))`
   >- (
     xapp>>xsimpl>>
+    rpt(first_x_assum (irule_at Any))>>xsimpl>>
+    qexists_tac`emp_vec`>>
+    qexists_tac`T`>>
+    qexists_tac`[]`>>
     CONJ_TAC >- EVAL_TAC>>
-    CONJ_TAC >- metis_tac[]>>
     CONJ_TAC >- EVAL_TAC>>
-    metis_tac[fetch "-" "emp_vec_v_thm"])
+    CONJ_TAC >- metis_tac[fetch "-" "emp_vec_v_thm"]>>
+    xsimpl)
   >- (
     xsimpl>>
-    metis_tac[ARRAY_refl])>>
+    metis_tac[ARRAY_W8ARRAY_refl])>>
   pop_assum mp_tac>> TOP_CASE_TAC>>gvs[]>>
   strip_tac>>
   rename1`check_subproofs_list xx`>>
   xlet`(POSTve
       (λv.
-        SEP_EXISTS fmlv' fmllsv'.
-        ARRAY fmlv' fmllsv' *
+        SEP_EXISTS fmlv' fmllsv' zerosv' zeros'.
+        ARRAY fmlv' fmllsv' * W8ARRAY zerosv' zeros' *
         &(
-          case check_subproofs_list xx T fmlls id id of
+          case check_subproofs_list xx T fmlls id id zeros of
             NONE => F
           | SOME res =>
             PAIR_TYPE (λl v.
               LIST_REL (OPTION_TYPE bconstraint_TYPE) l fmllsv' ∧
-              v = fmlv') NUM res v
+              v = fmlv')
+            (PAIR_TYPE NUM (λl v. l = zeros' ∧ v = zerosv'  ∧ EVERY (λw. w = 0w) zeros') ) res v
           ))
       (λe.
-        SEP_EXISTS fmlv' fmllsv'.
-        ARRAY fmlv' fmllsv' *
+        SEP_EXISTS fmlv' fmllsv' zerosv' zeros'.
+        ARRAY fmlv' fmllsv' * W8ARRAY zerosv' zeros' *
         & (Fail_exn e ∧
-          check_subproofs_list xx T fmlls id id = NONE)))`
+          check_subproofs_list xx T fmlls id id zeros = NONE)))`
   >- (
     xapp>>xsimpl>>
     CONJ_TAC>-EVAL_TAC>>
     metis_tac[])
   >- (
     xsimpl>>
-    metis_tac[ARRAY_refl])>>
+    metis_tac[ARRAY_W8ARRAY_refl])>>
   pop_assum mp_tac>> TOP_CASE_TAC>>fs[]>>
-  Cases_on`x'`>>fs[PAIR_TYPE_def]>>
+  qmatch_goalsub_rename_tac`PAIR_TYPE _ _ xxx _`>>
+  PairCases_on`xxx`>>fs[PAIR_TYPE_def]>>
   strip_tac>>
   xmatch>>
   rpt xlet_autop>>
@@ -3205,10 +3657,10 @@ Proof
     rpt xlet_autop>>
     xcon>>xsimpl>>
     fs[PAIR_TYPE_def]>>
-    metis_tac[ARRAY_refl])>>
+    metis_tac[ARRAY_W8ARRAY_refl])>>
   rpt xlet_autop>>
   xraise>> xsimpl>>
-  metis_tac[ARRAY_refl,Fail_exn_def]
+  metis_tac[ARRAY_W8ARRAY_refl,Fail_exn_def]
 QED
 
 val _ = register_type ``:proof_conf``
@@ -3346,17 +3798,6 @@ val res = translate err_obj_check_string_def;
 val res = translate npbc_checkTheory.eq_obj_def;
 val res = translate npbc_checkTheory.check_eq_obj_def;
 
-Definition w8z_def:
-  w8z = (0w: word8)
-End
-
-Definition w8o_def:
-  w8o = (1w: word8)
-End
-
-val w8z_v_thm = translate w8z_def;
-val w8o_v_thm = translate w8o_def;
-
 val fold_update_resize_bitset = process_topdecs`
   fun fold_update_resize_bitset ls acc =
     case ls of
@@ -3459,24 +3900,25 @@ Proof
 QED
 
 val check_cstep_arr = process_topdecs`
-  fun check_cstep_arr lno cstep fml inds vimap vomap pc =
+  fun check_cstep_arr lno cstep fml zeros inds vimap vomap pc =
   case cstep of
     Dom c s pfs idopt => (
     case get_ord pc of None =>
       raise Fail (format_failure lno "no order loaded for dominance step")
     | Some spo =>
       case check_dom_arr lno spo (get_obj pc)
-        fml inds (get_id pc) c (mk_subst s) pfs idopt of
-        (fml',(rinds,id')) =>
+        fml inds (get_id pc) c (mk_subst s) pfs idopt zeros of
+        (fml',(rinds,(id',zeros'))) =>
       (Array.updateResize fml' None id' (Some (c,get_tcb pc)),
+       (zeros',
        (sorted_insert id' rinds,
        (update_vimap vimap id' (fst c),
-        (vomap, set_id pc (id'+1))))))
+        (vomap, set_id pc (id'+1)))))))
   | Sstep sstep => (
     case check_sstep_arr lno sstep (get_ord pc) (get_obj pc)
-      (get_tcb pc) fml inds (get_id pc) vimap vomap of
-      (fml',(inds',(vimap',id'))) =>
-      (fml',(inds',(vimap',(vomap, set_id pc id')))))
+      (get_tcb pc) fml inds (get_id pc) vimap vomap zeros of
+      (fml',(inds',(vimap',(id',zeros')))) =>
+      (fml',(zeros',(inds',(vimap',(vomap, set_id pc id'))))))
   | Checkeddelete n s pfs idopt => (
     if check_tcb_idopt_pc pc idopt
     then
@@ -3487,36 +3929,36 @@ val check_cstep_arr = process_topdecs`
           case
             check_red_arr lno (get_ord pc) (get_obj pc) True
               (get_tcb pc) fml inds (get_id pc)
-              c s pfs idopt vimap vomap of
-              (fml',(inds',(vimap',id'))) =>
-              (fml',(inds',(vimap',(vomap,set_id pc id'))))))
+              c s pfs idopt vimap vomap zeros of
+              (fml',(inds',(vimap',(id',zeros')))) =>
+              (fml',(zeros',(inds',(vimap',(vomap,set_id pc id')))))))
     else raise Fail
       (format_failure lno
         "invalid proof state for checked deletion"))
   | Uncheckeddelete ls => (
     if check_tcb_ord pc then
       (list_delete_arr ls fml;
-        (fml, (inds, (vimap, (vomap, set_chk pc False)))))
+        (fml, (zeros, (inds, (vimap, (vomap, set_chk pc False))))))
     else
       case all_core_arr fml inds [] of None =>
         raise Fail (format_failure lno
         "not all constraints in core")
       | Some inds' =>
         (list_delete_arr ls fml;
-          (fml, (inds', (vimap, (vomap, set_chk pc False))))))
+          (fml, (zeros, (inds', (vimap, (vomap, set_chk pc False)))))))
   | Transfer ls => (
       let val fml' = core_from_inds_arr lno fml ls in
-        (fml', (inds, (vimap, (vomap, pc))))
+        (fml', (zeros, (inds, (vimap, (vomap, pc)))))
       end)
   | Strengthentocore b => (
     let val inds' = reindex_arr fml inds in
       if b
       then (
         let val fml' = core_from_inds_arr lno fml inds' in
-          (fml', (inds', (vimap, (vomap, set_tcb pc b))))
+          (fml',(zeros, (inds', (vimap, (vomap, set_tcb pc b)))))
         end)
       else
-        (fml,(inds', (vimap, (vomap, set_tcb pc b))))
+        (fml, (zeros, (inds', (vimap, (vomap, set_tcb pc b)))))
     end)
   | Loadorder nn xs =>
     let val inds' = reindex_arr fml inds in
@@ -3526,7 +3968,7 @@ val check_cstep_arr = process_topdecs`
     | Some ord' =>
       if List.length xs = List.length (fst (snd ord')) then
         let val fml' = core_from_inds_arr lno fml inds' in
-        (fml', (inds', (vimap, (vomap, set_ord pc (Some (ord',xs))))))
+        (fml', (zeros, (inds', (vimap, (vomap, set_ord pc (Some (ord',xs)))))))
         end
       else
         raise Fail
@@ -3536,11 +3978,11 @@ val check_cstep_arr = process_topdecs`
     (case get_ord pc of None =>
      raise Fail (format_failure lno ("no order loaded"))
     | Some spo =>
-      (fml,(inds,(vimap,(vomap,set_ord pc None)))))
+      (fml,(zeros,(inds,(vimap,(vomap,set_ord pc None))))))
   | Storeorder name spo ws pfsr pfst =>
     if check_storeorder spo ws pfst pfsr
     then
-     (fml, (inds, (vimap, (vomap, set_orders pc ((name,spo)::get_orders pc)))))
+     (fml, (zeros, (inds, (vimap, (vomap, set_orders pc ((name,spo)::get_orders pc))))))
     else
       raise Fail (format_failure lno ("invalid order definition"))
   | Obj w mi bopt => (
@@ -3559,23 +4001,24 @@ val check_cstep_arr = process_topdecs`
           val id = get_id pc
           val c = model_improving obj new in
           (Array.updateResize fml None id (Some (c,True)),
+           (zeros,
            (sorted_insert id inds,
            (update_vimap vimap id (fst c),
            (vomap,
-            obj_update pc (id+1) bound' dbound'))))
+            obj_update pc (id+1) bound' dbound')))))
         end
       else
-        (fml, (inds, (vimap, (vomap, obj_update pc (get_id pc) bound' dbound'))))
+        (fml, (zeros, (inds, (vimap, (vomap, obj_update pc (get_id pc) bound' dbound')))))
     end
     )
   | Changeobj b fc' pfs =>
     (case check_change_obj_arr lno b fml
-      (get_id pc) (get_obj pc) fc' pfs of
-      (fml',(fc',id')) =>
-        (fml', (inds, (vimap, (mk_vomap_arr (String.size vomap) fc', change_obj_update pc id' fc')))))
+      (get_id pc) (get_obj pc) fc' pfs zeros of
+      (fml',(fc',(id',zeros'))) =>
+        (fml', (zeros', (inds, (vimap, (mk_vomap_arr (String.size vomap) fc', change_obj_update pc id' fc'))))))
   | Checkobj fc' =>
     if check_eq_obj (get_obj pc) fc'
-    then (fml, (inds, (vimap, (vomap, pc))))
+    then (fml, (zeros, (inds, (vimap, (vomap, pc)))))
     else
       raise Fail (format_failure lno
         (err_obj_check_string (get_obj pc) fc'))
@@ -3610,34 +4053,36 @@ Theorem check_cstep_arr_spec:
   (LIST_TYPE NUM) inds indsv ∧
   NPBC_CHECK_PROOF_CONF_TYPE pc pcv ∧
   vimap_TYPE vimap vimapv ∧
-  vomap_TYPE vomap vomapv
+  vomap_TYPE vomap vomapv ∧
+  EVERY (λw. w = 0w) zeros
   ⇒
   app (p : 'ffi ffi_proj)
     ^(fetch_v "check_cstep_arr" (get_ml_prog_state()))
-    [lnov; cstepv; fmlv; indsv; vimapv; vomapv; pcv]
-    (ARRAY fmlv fmllsv)
+    [lnov; cstepv; fmlv; zerosv; indsv; vimapv; vomapv; pcv]
+    (ARRAY fmlv fmllsv * W8ARRAY zerosv zeros)
     (POSTve
       (λv.
-        SEP_EXISTS fmlv' fmllsv'.
-        ARRAY fmlv' fmllsv' *
+        SEP_EXISTS fmlv' fmllsv' zerosv' zeros'.
+        ARRAY fmlv' fmllsv' * W8ARRAY zerosv' zeros' *
         &(
-          case check_cstep_list cstep fmlls inds vimap vomap pc of
+          case check_cstep_list cstep fmlls zeros inds vimap vomap pc of
             NONE => F
           | SOME res =>
             PAIR_TYPE (λl v.
               LIST_REL (OPTION_TYPE bconstraint_TYPE) l fmllsv' ∧
               v = fmlv')
+              (PAIR_TYPE (λl v. l = zeros' ∧ v = zerosv'  ∧ EVERY (λw. w = 0w) zeros')
               (PAIR_TYPE (LIST_TYPE NUM)
                 (PAIR_TYPE (vimap_TYPE)
                   (PAIR_TYPE (vomap_TYPE)
-                  NPBC_CHECK_PROOF_CONF_TYPE)))
+                  NPBC_CHECK_PROOF_CONF_TYPE))))
                 res v
           ))
       (λe.
-        SEP_EXISTS fmlv' fmllsv'.
-        ARRAY fmlv' fmllsv' *
+        SEP_EXISTS fmlv' fmllsv' zerosv' zeros'.
+        ARRAY fmlv' fmllsv' * W8ARRAY zerosv' zeros' *
         & (Fail_exn e ∧
-          check_cstep_list cstep fmlls inds vimap vomap pc = NONE)))
+          check_cstep_list cstep fmlls zeros inds vimap vomap pc = NONE)))
 Proof
   rw[]>>
   xcf "check_cstep_arr" (get_ml_prog_state ())>>
@@ -3651,25 +4096,32 @@ Proof
     >- (
       rpt xlet_autop>>
       xraise>> xsimpl>>
-      metis_tac[Fail_exn_def,ARRAY_refl])>>
+      metis_tac[Fail_exn_def,ARRAY_W8ARRAY_refl])>>
     rpt xlet_autop>>
     xlet_auto >-
       (xsimpl>> simp (eq_lemmas()))>>
     rpt xlet_autop>>
-    fs[get_id_def,get_obj_def]
+    fs[get_id_def,get_obj_def]>>
+    xlet_auto
+    >- (
+      xsimpl>>
+      metis_tac[ARRAY_W8ARRAY_refl])
     >- (
       xsimpl>>
       simp[check_dom_list_def]>>
       rw[]>>
-      qmatch_goalsub_abbrev_tac`ARRAY A B`>>
-      qexists_tac`A`>>qexists_tac`B`>>xsimpl>>
+      qmatch_goalsub_abbrev_tac`W8ARRAY C D * ARRAY A B`>>
+      qexists_tac`A`>>qexists_tac`B`>>
+      qexists_tac`C`>>qexists_tac`D`>>
+      xsimpl>>
       fs[do_dom_check_def,AllCaseEqs()])>>
-    pop_assum mp_tac>>TOP_CASE_TAC>>strip_tac>>
-    PairCases_on`x'`>>fs[PAIR_TYPE_def]>>
+    pop_assum mp_tac>>TOP_CASE_TAC>>
+    qmatch_goalsub_rename_tac`PAIR_TYPE _ _ xxx _`>>
+    strip_tac>>
+    PairCases_on`xxx`>>fs[PAIR_TYPE_def]>>
     xmatch>>
     rpt xlet_autop>>
     gvs[check_dom_list_def,AllCaseEqs()]>>
-    xlet_auto>>
     xcon>>xsimpl>>
     simp[PAIR_TYPE_def,OPTION_TYPE_def]>>
     qmatch_goalsub_abbrev_tac`ARRAY _ A`>>
@@ -3682,10 +4134,14 @@ Proof
   >- ( (* Sstep *)
     xmatch>>
     rpt xlet_autop>>
-    fs[get_tcb_def,get_id_def,get_obj_def,get_ord_def]
+    fs[get_tcb_def,get_id_def,get_obj_def,get_ord_def]>>
+    xlet_auto
     >- (
       xsimpl>>
-      metis_tac[ARRAY_refl])>>
+      metis_tac[ARRAY_W8ARRAY_refl])
+    >- (
+      xsimpl>>
+      metis_tac[ARRAY_W8ARRAY_refl])>>
     pop_assum mp_tac>>
     TOP_CASE_TAC>>
     PairCases_on`x`>>simp[PAIR_TYPE_def]>>rw[]>>
@@ -3701,16 +4157,18 @@ Proof
       rpt xlet_autop>>
       xraise>>xsimpl>>
       fs[Fail_exn_def]>>
-      metis_tac[ARRAY_refl])>>
+      metis_tac[ARRAY_W8ARRAY_refl])>>
     rpt xlet_autop>>
     xlet`POSTv v.
-      ARRAY fmlv fmllsv *
+      ARRAY fmlv fmllsv * W8ARRAY zerosv zeros *
       &(
         OPTION_TYPE constraint_TYPE
         (lookup_core_only_list T fmlls n) v)`
     >- (
       xapp>>
-      xsimpl)>>
+      xsimpl>>
+      rpt (first_x_assum (irule_at Any))>>
+      qexists_tac`T`>>xsimpl)>>
     fs[check_tcb_idopt_pc_def]>>
     Cases_on`lookup_core_only_list T fmlls n`>>
     fs[OPTION_TYPE_def]>>xmatch
@@ -3718,37 +4176,35 @@ Proof
       rpt xlet_autop>>
       xraise>>xsimpl>>
       fs[Fail_exn_def]>>
-      metis_tac[ARRAY_refl])>>
+      metis_tac[ARRAY_W8ARRAY_refl])>>
     rpt xlet_autop>>
     fs[get_id_def,get_tcb_def,get_obj_def,get_ord_def]>>
-    rename1`check_red_list ord obj T pc.tcb (delete_list n fmlls)
-      inds pc.id c s pfs idopt vimap vomap`>>
+    rename1`check_red_list ord obj T pc.tcb (delete_list n fmlls) inds pc.id c s pfs idopt vimap vomap zeros`>>
     xlet`POSTve
       (λv.
-        SEP_EXISTS fmlv' fmllsv'.
-        ARRAY fmlv' fmllsv' *
+        SEP_EXISTS fmlv' fmllsv' zerosv' zeros'.
+        ARRAY fmlv' fmllsv' * W8ARRAY zerosv' zeros' *
         &(
-        case check_red_list ord obj T pc.tcb (delete_list n fmlls)
-          inds pc.id c s pfs idopt vimap vomap of NONE => F
+        case check_red_list ord obj T pc.tcb (delete_list n fmlls) inds pc.id c s pfs idopt vimap vomap zeros of NONE => F
         | SOME res =>
           PAIR_TYPE (λl v.
             LIST_REL (OPTION_TYPE bconstraint_TYPE) l fmllsv' ∧
             v = fmlv') (PAIR_TYPE (LIST_TYPE NUM)
-              (PAIR_TYPE vimap_TYPE NUM)) res v
+              (PAIR_TYPE vimap_TYPE
+              (PAIR_TYPE NUM (λl v. l = zeros' ∧ v = zerosv'  ∧ EVERY (λw. w = 0w) zeros') ))) res v
         ))
       (λe.
-        SEP_EXISTS fmlv' fmllsv'.
-        ARRAY fmlv' fmllsv' *
+        SEP_EXISTS fmlv' fmllsv' zerosv' zeros'.
+        ARRAY fmlv' fmllsv' * W8ARRAY zerosv' zeros' *
         & (Fail_exn e ∧
-          check_red_list ord obj T pc.tcb (delete_list n fmlls)
-            inds pc.id c s pfs idopt vimap vomap = NONE))`
+          check_red_list ord obj T pc.tcb (delete_list n fmlls) inds pc.id c s pfs idopt vimap vomap zeros = NONE))`
     >- (
       xapp>>xsimpl>>
       CONJ_TAC >- EVAL_TAC>>
       metis_tac[])
     >- (
       xsimpl>>
-      metis_tac[ARRAY_refl])>>
+      metis_tac[ARRAY_W8ARRAY_refl])>>
     pop_assum mp_tac>>
     TOP_CASE_TAC>>fs[]>>
     PairCases_on`x`>>fs[PAIR_TYPE_def]>>
@@ -3763,7 +4219,9 @@ Proof
     >- (
       rpt xlet_autop>>
       xlet`POSTv v.
-        ARRAY fmlv fmllsv' * &NPBC_CHECK_PROOF_CONF_TYPE (set_chk pc F) v`
+        ARRAY fmlv fmllsv' *
+        W8ARRAY zerosv zeros *
+        &NPBC_CHECK_PROOF_CONF_TYPE (set_chk pc F) v`
       >- (
         xapp>>xsimpl>>
         rw[]>>
@@ -3774,8 +4232,10 @@ Proof
       xcon>>xsimpl>>
       fs[]>>
       fs[PAIR_TYPE_def,set_chk_def]>>
-      metis_tac[ARRAY_refl])>>
-    xlet`POSTv v. ARRAY fmlv fmllsv * &(LIST_TYPE NUM [] v)`
+      metis_tac[ARRAY_W8ARRAY_refl])>>
+    xlet`POSTv v. ARRAY fmlv fmllsv *
+      W8ARRAY zerosv zeros *
+      &(LIST_TYPE NUM [] v)`
     >- (
       xcon>>xsimpl>>
       EVAL_TAC)>>
@@ -3785,10 +4245,12 @@ Proof
     >- (
       rpt xlet_autop>>
       xraise>>xsimpl>>
-      metis_tac[Fail_exn_def,ARRAY_refl])>>
+      metis_tac[Fail_exn_def,ARRAY_W8ARRAY_refl])>>
     rpt xlet_autop>>
     xlet`POSTv v.
-        ARRAY fmlv fmllsv' * &NPBC_CHECK_PROOF_CONF_TYPE (set_chk pc F) v`
+        ARRAY fmlv fmllsv' *
+        W8ARRAY zerosv zeros *
+        &NPBC_CHECK_PROOF_CONF_TYPE (set_chk pc F) v`
     >- (
       xapp>>xsimpl>>
       rw[]>>
@@ -3803,31 +4265,38 @@ Proof
     xsimpl)
   >- ( (* Transfer *)
     xmatch>>
-    xlet_autop
+    xlet_auto
     >- (
       xsimpl>>
-      metis_tac[ARRAY_refl])>>
+      metis_tac[ARRAY_refl])
+    >- (
+      xsimpl>>
+      metis_tac[ARRAY_W8ARRAY_refl])>>
     rpt xlet_autop>>
     xcon>>every_case_tac>>fs[]>>xsimpl>>
     simp[PAIR_TYPE_def]>>
-    metis_tac[ARRAY_refl])
+    metis_tac[ARRAY_W8ARRAY_refl])
   >- ( (* StrengthenToCore *)
     xmatch>>
     rpt xlet_autop>>
     xif
     >- (
-      xlet_autop>>xsimpl
-      >-
-        (metis_tac[ARRAY_refl])>>
+      xlet_auto
+      >- (
+        xsimpl>>
+        metis_tac[ARRAY_refl])
+      >- (
+        xsimpl>>
+        metis_tac[ARRAY_W8ARRAY_refl])>>
       pop_assum mp_tac>>TOP_CASE_TAC>>strip_tac>>
       rpt xlet_autop>>
       xcon>>xsimpl>>
       fs[PAIR_TYPE_def,set_tcb_def]>>
-      metis_tac[ARRAY_refl])>>
+      metis_tac[ARRAY_W8ARRAY_refl])>>
     rpt xlet_autop>>
     xcon>>xsimpl>>
     fs[PAIR_TYPE_def,set_tcb_def]>>
-    metis_tac[ARRAY_refl])
+    metis_tac[ARRAY_W8ARRAY_refl])
   >- ( (* LoadOrder*)
     xmatch>>
     rpt xlet_autop>>
@@ -3836,28 +4305,34 @@ Proof
     >- (
       rpt xlet_autop>>
       xraise>> xsimpl>>
-      metis_tac[Fail_exn_def,ARRAY_refl])>>
+      metis_tac[Fail_exn_def,ARRAY_W8ARRAY_refl])>>
     rpt xlet_autop>>
     reverse xif
     >- (
       rpt xlet_autop>>
       xraise>> xsimpl>>
-      metis_tac[Fail_exn_def,ARRAY_refl])>>
-    rpt xlet_autop
+      metis_tac[Fail_exn_def,ARRAY_W8ARRAY_refl])>>
+    rpt xlet_autop>>
+    xlet_auto
     >- (
       xsimpl>>
-      metis_tac[ARRAY_refl])>>
-    xlet`POSTv v. ARRAY fmlv' fmllsv' *
+      metis_tac[ARRAY_refl])
+    >- (
+      xsimpl>>
+      metis_tac[ARRAY_W8ARRAY_refl])>>
+    rpt xlet_autop>>
+    xlet`POSTv v. ARRAY fmlv' fmllsv' * W8ARRAY zerosv zeros *
       &NPBC_CHECK_PROOF_CONF_TYPE (set_ord pc (SOME (x,l))) v`
     >- (
       xapp>>xsimpl>>
       asm_exists_tac>>simp[]>>
-      qexists_tac`SOME (x,l)`>>simp[OPTION_TYPE_def,PAIR_TYPE_def])>>
+      qexists_tac`SOME (x,l)`>>
+      simp[OPTION_TYPE_def,PAIR_TYPE_def])>>
     rpt xlet_autop>>
     xcon>>xsimpl>>
     every_case_tac>>
     gvs[AllCaseEqs(),PAIR_TYPE_def,OPTION_TYPE_def,set_ord_def]>>
-    metis_tac[ARRAY_refl])
+    metis_tac[ARRAY_W8ARRAY_refl])
   >- ( (* UnloadOrder *)
     xmatch>>
     xlet_autop>>fs[get_ord_def]>>
@@ -3866,9 +4341,9 @@ Proof
     >- (
       rpt xlet_autop>>
       xraise>> xsimpl>>
-      metis_tac[Fail_exn_def,ARRAY_refl])>>
+      metis_tac[Fail_exn_def,ARRAY_W8ARRAY_refl])>>
     rpt xlet_autop>>
-    xlet`POSTv v. ARRAY fmlv fmllsv *
+    xlet`POSTv v. ARRAY fmlv fmllsv * W8ARRAY zerosv zeros *
       &NPBC_CHECK_PROOF_CONF_TYPE (set_ord pc NONE) v`
     >- (
       xapp>>xsimpl>>
@@ -3877,7 +4352,7 @@ Proof
     rpt xlet_autop>>
     xcon>>xsimpl>>
     fs[PAIR_TYPE_def,OPTION_TYPE_def,set_ord_def]>>
-    metis_tac[ARRAY_refl])
+    metis_tac[ARRAY_W8ARRAY_refl])
   >- ( (* StoreOrder *)
     xmatch>>
     xlet_autop>>
@@ -3887,11 +4362,11 @@ Proof
       xraise>>xsimpl>>
       every_case_tac>>
       gvs[check_storeorder_def,Fail_exn_def,AllCaseEqs()]>>
-      metis_tac[ARRAY_refl])>>
+      metis_tac[ARRAY_W8ARRAY_refl])>>
     gvs[check_storeorder_def]>>
     every_case_tac>>fs[]>>
     rpt xlet_autop>>
-    xlet`POSTv v. ARRAY fmlv fmllsv *
+    xlet`POSTv v. ARRAY fmlv fmllsv * W8ARRAY zerosv zeros *
       &NPBC_CHECK_PROOF_CONF_TYPE (set_orders pc ((m,p')::pc.orders)) v`
     >- (
       xapp>>xsimpl>>simp[set_orders_def]>>
@@ -3902,7 +4377,8 @@ Proof
     xcon>>xsimpl>>
     fs[PAIR_TYPE_def,OPTION_TYPE_def,LIST_TYPE_def,set_orders_def]>>
     asm_exists_tac>>simp[]>>
-    metis_tac[ARRAY_refl])
+    xsimpl>>
+    metis_tac[ARRAY_W8ARRAY_refl])
   >- ( (* Obj *)
     xmatch>>
     rpt xlet_autop>>
@@ -3915,7 +4391,7 @@ Proof
       rpt xlet_autop>>
       xraise>>
       xsimpl>>
-      metis_tac[Fail_exn_def,ARRAY_refl])>>
+      metis_tac[Fail_exn_def,ARRAY_W8ARRAY_refl])>>
     rpt xlet_autop>>
     pairarg_tac>>
     fs[get_chk_def,get_bound_def,get_dbound_def,PAIR_TYPE_def]>>
@@ -3928,10 +4404,9 @@ Proof
       `pc with <|id := pc.id; bound := bound'; dbound := dbound'|>
         = pc with <|bound := bound'; dbound := dbound'|>` by
        fs[npbc_checkTheory.proof_conf_component_equality]>>
-      metis_tac[ARRAY_refl])
+      metis_tac[ARRAY_W8ARRAY_refl])
     >- ( (* model improving *)
       rpt xlet_autop>>
-      xlet_auto>>
       xcon>>xsimpl>>
       simp[PAIR_TYPE_def,OPTION_TYPE_def]>>
       qmatch_goalsub_abbrev_tac`ARRAY _ A`>>
@@ -3943,11 +4418,16 @@ Proof
       EVAL_TAC))
   >- ( (* ChangeObj *)
     xmatch>>
-    rpt xlet_autop
+    rpt xlet_autop>>
+    xlet_auto
     >- (
       xsimpl>>
       fs[get_obj_def,get_id_def]>>
-      metis_tac[ARRAY_refl])>>
+      metis_tac[ARRAY_W8ARRAY_refl])
+    >- (
+      xsimpl>>
+      fs[get_obj_def,get_id_def]>>
+      metis_tac[ARRAY_W8ARRAY_refl])>>
     pop_assum mp_tac>> every_case_tac>>
     fs[get_id_def,get_obj_def]>>
     rw[PAIR_TYPE_def]>>
@@ -3965,10 +4445,10 @@ Proof
       rpt xlet_autop>>
       xcon>>xsimpl>>
       simp[PAIR_TYPE_def]>>
-      metis_tac[ARRAY_refl])>>
+      metis_tac[ARRAY_W8ARRAY_refl])>>
     rpt xlet_autop>>
     xraise>>xsimpl>>
-    metis_tac[Fail_exn_def,ARRAY_refl])
+    metis_tac[Fail_exn_def,ARRAY_W8ARRAY_refl])
 QED
 
 val check_implies_fml_arr = process_topdecs`
